Refactor DEFINE-HASH-TABLE$A

books/projects/atomic-stobjs/constructors/hash-table-a.lisp
@@ -39,17 +39,35 @@
 (include-book "../utilities/top")
 
 
+;;;; `SET::EQUIV'
+(defun set::equiv (x y)
+  (declare (xargs :guard (and (set::setp x)
+                              (set::setp y))))
+  (mbe :logic (equal (set::sfix x)
+                     (set::sfix y))
+       :exec (equal x y)))
+
+(defequiv set::equiv)
+
+(defcong set::equiv equal (set::sfix x) 1)
+
+(defthm set::sfix-mode-set-equiv
+  (set::equiv (set::sfix x) x))
+
+
 ;;;; `DEFINE-HASH-TABLE$A'
 (defmacro define-hash-table$a
     (hash-table test
      &key
        (key-recognizer 'nil)
        (key-fixer 'nil)
+       (key-equiv 'equal)
        (key 'nil)
        (%key 'nil)
        (default-key 'nil)
        (val-recognizer 'nil)
        (val-fixer 'nil)
+       (val-equiv 'equal)
        (val 'nil)
        (%val 'nil)
        (default-val 'nil)
@@ -61,6 +79,7 @@
        (recognizer 'nil)
        (creator 'nil)
        (fixer 'nil)
+       (equiv 'nil)
        (accessor 'nil)
        (updater 'nil)
        (boundp 'nil)
@@ -71,6 +90,7 @@
        (init 'nil)
        (keysp 'nil)
        (keys-fix 'nil)
+       (keys-equiv 'nil)
        (keys 'nil)
        (keys-set 'nil)
 
@@ -82,9 +102,11 @@
                               (member test '(eq eql hons-equal equal) :test 'eq)
                               (symbol-listp (list key-recognizer
                                                   key-fixer
+                                                  key-equiv
                                                   key
                                                   val-recognizer
                                                   val-fixer
+                                                  val-equiv
                                                   val))
                               (or (and (not key-recognizer)
                                        (not key-fixer)
@@ -99,6 +121,7 @@
                               (booleanp copyable)
                               (symbol-listp (list recognizer
                                                   fixer
+                                                  equiv
                                                   creator
                                                   accessor
                                                   updater
@@ -110,13 +133,15 @@
                                                   init
                                                   keysp
                                                   keys-fix
+                                                  keys-equiv
                                                   keys
                                                   keys-set))
                               (or copyable
-                                  (and (not keysp)
+                                  (and (not keys)
+                                       (not keys-set)
+                                       (not keysp)
                                        (not keys-fix)
-                                       (not keys)
-                                       (not keys-set)))
+                                       (not keys-equiv)))
                               (package-witness-p package-witness)
                               (booleanp debug))))
 
@@ -137,6 +162,7 @@
                         (symbolicate key "%" key)))
               (key-recognizer ',key-recognizer)
               (key-fixer ',key-fixer)
+              (key-equiv ',key-equiv)
               (default-key-name (symbolicate package-witness "*" hash-table "-DEFAULT-KEY*"))
               (default-key default-key-name)
 
@@ -165,6 +191,10 @@
                             (third (second stobj$a-property)))
                            (t
                             (cdr (assoc val (table-alist 'fixer world))))))
+              (val-equiv (cond
+                           (',val-equiv)
+                           (stobj$a-property
+                            (fourth (second stobj$a-property)))))
               (default-val-name (symbolicate package-witness "*" hash-table "-DEFAULT-VAL*"))
               (default-val (if val-creator
                                `(,val-creator)
@@ -179,6 +209,7 @@
               (recognizer ',recognizer)
               (creator ',creator)
               (fixer ',fixer)
+              (equiv ',equiv)
               (accessor ',accessor)
               (updater ',updater)
               (boundp ',boundp)
@@ -189,6 +220,7 @@
               (init ',init)
               (keysp ',keysp)
               (keys-fix ',keys-fix)
+              (keys-equiv ',keys-equiv)
               (keys ',keys)
               (keys-set ',keys-set)
 
@@ -199,6 +231,8 @@
                            (symbolicate package-witness "CREATE-" hash-table)))
               (fixer (or fixer
                          (symbolicate package-witness hash-table "-FIX")))
+              (equiv (or equiv
+                         (symbolicate package-witness hash-table "-EQUIV")))
               (accessor (or accessor
                             (symbolicate package-witness hash-table "-GET")))
               (updater (or updater
@@ -215,10 +249,21 @@
                          (symbolicate package-witness hash-table "-CLEAR")))
               (init (or init
                         (symbolicate package-witness hash-table "-INIT")))
-              (keysp (or keysp
-                         (symbolicate package-witness hash-table "-KEYS-P")))
-              (keys-fix (or keys-fix
-                            (symbolicate package-witness hash-table "-KEYS-FIX")))
+              (keysp (if (and copyable
+                              key-recognizer)
+                         (or keysp
+                             (symbolicate package-witness hash-table "-KEYS-P"))
+                         'set::setp))
+              (keys-fix (if (and copyable
+                                 key-recognizer)
+                            (or keys-fix
+                                (symbolicate package-witness hash-table "-KEYS-FIX"))
+                            'set::sfix))
+              (keys-equiv (if (and copyable
+                                   key-recognizer)
+                              (or keys-equiv
+                                  (symbolicate package-witness hash-table "-KEYS-EQUIV"))
+                              'set::equiv))
               (keys (or keys
                         (symbolicate package-witness hash-table "-KEYS")))
               (keys-set (or keys-set
@@ -273,8 +318,41 @@
                         `((defconst ,default-val-name ',',default-val)))))
 
               ;; Theorem Names
-              (key-fixer-rw (symbolicate "ATOMIC-STOBJS" key-fixer "-RW-1"))
-              (val-fixer-rw (symbolicate "ATOMIC-STOBJS" val-fixer "-RW-2"))
+              (key-recognizer-constraints (symbolicate "ATOMIC-STOBJS" key-recognizer "-CONSTRAINTS-1"))
+              (key-fixer-constraints (symbolicate "ATOMIC-STOBJS" key-fixer "-CONSTRAINTS-1"))
+              (key-equiv-constraints (symbolicate "ATOMIC-STOBJS" key-equiv "-CONSTRAINTS-1"))
+              (val-recognizer-constraints (symbolicate "ATOMIC-STOBJS" val-recognizer "-CONSTRAINTS-2"))
+              (val-fixer-constraints (symbolicate "ATOMIC-STOBJS" val-fixer "-CONSTRAINTS-2"))
+              (val-equiv-constraints (symbolicate "ATOMIC-STOBJS" val-equiv "-CONSTRAINTS-2"))
+
+              (hash-table-constraints (symbolicate package-witness hash-table "-CONSTRAINTS"))
+
+              (keysp-tp (symbolicate package-witness keysp "-TP"))
+              (keysp-cr (symbolicate package-witness keysp "-CR"))
+              (keysp-def (symbolicate package-witness keysp "-DEF"))
+              (setp-when-keysp (symbolicate package-witness "SETP-WHEN-" keysp))
+              (keysp-when-emptyp (symbolicate package-witness keysp "-WHEN-EMPTYP"))
+              (keysp-of-keys-fix (symbolicate package-witness keysp "-OF-" keys-fix))
+              (keysp-of-keys (symbolicate package-witness (if key-recognizer keysp "SETP") "-OF-" keys))
+              (keysp-of-sfix (symbolicate package-witness keysp "-OF-SFIX"))
+              (key-recognizer-of-head-when-keysp (symbolicate package-witness key-recognizer "-OF-HEAD-WHEN-" keysp))
+              (keysp-of-tail-when-keysp (symbolicate package-witness keysp "-OF-TAIL-WHEN-" keysp))
+              (keysp-of-insert (symbolicate package-witness keysp "-OF-INSERT"))
+              (in-when-keysp (symbolicate package-witness "IN-WHEN-" keysp))
+              (in-when-keysp-split (symbolicate package-witness in-when-keysp "-SPLIT"))
+              (subset-when-keysp (symbolicate package-witness keysp "-WHEN-SUBSET"))
+              (keysp-of-delete (symbolicate package-witness keysp "-OF-DELETE"))
+              (keysp-of-union (symbolicate package-witness keysp "-OF-UNION"))
+              (keysp-of-intersect (symbolicate package-witness keysp "-OF-INTERSECT"))
+              (keysp-of-difference (symbolicate package-witness keysp "-OF-DIFFERENCE"))
+
+              (keys-fix-tp (symbolicate package-witness keys-fix "-TP"))
+              (keys-fix-when-keysp (symbolicate package-witness keys-fix "-WHEN-" keysp))
+              (keys-fix-when-not-keysp (symbolicate package-witness keys-fix "-WHEN-NOT-" keysp))
+
+              (keys-equiv-tp (symbolicate package-witness keys-equiv "-TP"))
+              (keys-fix-mod-keys-equiv (symbolicate package-witness keys-fix "-MOD-" keys-equiv))
+              (keys-equiv-when-not-keysp (symbolicate package-witness keys-equiv "-WHEN-NOT-" keysp))
 
               (recognizer-tp (symbolicate package-witness recognizer "-TP"))
               (recognizer-cr (symbolicate package-witness recognizer "-CR"))
@@ -288,12 +366,14 @@
               (fixer-when-recognizer (symbolicate package-witness fixer "-WHEN-" recognizer))
               (fixer-when-not-recognizer (symbolicate package-witness fixer "-WHEN-NOT-" recognizer))
 
+              (equiv-tp (symbolicate package-witness equiv "-TP"))
+              (fixer-mod-equiv (symbolicate package-witness fixer "-MOD-" equiv))
+              (equiv-when-not-recognizer (symbolicate package-witness equiv "-WHEN-NOT-" recognizer))
+
               (val-recognizer-of-accessor (symbolicate package-witness val-recognizer "-OF-" accessor))
               (accessor-when-not-key-recognizer (symbolicate package-witness accessor "-WHEN-NOT-" key-recognizer))
               (accessor-when-not-recognizer (symbolicate package-witness accessor "-WHEN-NOT-" recognizer))
               (accessor-of-creator (symbolicate package-witness accessor "-OF-" creator))
-              (accessor-of-key-fixer (symbolicate package-witness accessor "-OF-" key-fixer))
-              (accessor-of-fixer (symbolicate package-witness accessor "-OF-" fixer))
               (accessor-of-updater (symbolicate package-witness accessor "-OF-" updater))
               (accessor-of-updater-same (symbolicate package-witness accessor-of-updater "-SAME"))
               (accessor-of-updater-diff (symbolicate package-witness accessor-of-updater "-DIFF"))
@@ -302,6 +382,7 @@
               (accessor-of-remover-same (symbolicate package-witness accessor-of-remover "-SAME"))
               (accessor-of-remover-diff (symbolicate package-witness accessor-of-remover "-DIFF"))
               (accessor-of-keys-set (symbolicate package-witness accessor "-OF-" keys-set))
+              (accessor-when-count-is-zero (symbolicate package-witness accessor "-WHEN-" count "-IS-ZERO"))
 
               (updater-tp (symbolicate package-witness updater "-TP"))
               (updater-when-not-key-recognizer (symbolicate package-witness updater "-WHEN-NOT-" key-recognizer))
@@ -313,19 +394,10 @@
                                                    (symbolicate package-witness updater-when-not-val-recognizer "-2")
                                                    updater-when-not-val-recognizer))
               (updater-when-not-recognizer (symbolicate package-witness updater "-WHEN-NOT-" recognizer))
-              (updater-of-key-fixer (symbolicate package-witness updater "-OF-" key-fixer))
-              (updater-of-val-fixer (symbolicate package-witness updater "-OF-" val-fixer))
-              (updater-of-key-fixer (if (eq updater-of-key-fixer updater-of-val-fixer)
-                                        (symbolicate package-witness updater-of-key-fixer "-1")
-                                        updater-of-key-fixer))
-              (updater-of-val-fixer (if (eq updater-of-key-fixer updater-of-val-fixer)
-                                        (symbolicate package-witness updater-of-val-fixer "-2")
-                                        updater-of-val-fixer))
-              (updater-of-fixer (symbolicate package-witness updater "-OF-" fixer))
               (updater-of-accessor (symbolicate package-witness updater "-OF-" accessor))
               (updater-of-accessor-when-boundp (symbolicate package-witness updater-of-accessor "-WHEN-" boundp))
-              (updater-of-accessor-when-not-boundp (symbolicate package-witness updater-of-accessor "-WHEN-NOT-" boundp))
               (updater-of-accessor-when-boundp-free (symbolicate package-witness updater-of-accessor-when-boundp "-FREE"))
+              (updater-of-accessor-when-not-boundp (symbolicate package-witness updater-of-accessor "-WHEN-NOT-" boundp))
               (updater-of-updater (symbolicate package-witness updater "-OF-" updater))
               (updater-of-updater-same (symbolicate package-witness updater-of-updater "-SAME"))
               (updater-of-updater-diff (symbolicate package-witness updater-of-updater "-DIFF"))
@@ -335,16 +407,14 @@
               (boundp-when-not-key-recognizer (symbolicate package-witness boundp "-WHEN-NOT-" key-recognizer))
               (boundp-when-not-recognizer (symbolicate package-witness boundp "-WHEN-NOT-" recognizer))
               (boundp-of-creator (symbolicate package-witness boundp "-OF-" creator))
-              (boundp-of-key-fixer (symbolicate package-witness boundp "-OF-" key-fixer))
-              (boundp-of-fixer (symbolicate package-witness boundp "-OF-" fixer))
               (boundp-of-updater (symbolicate package-witness boundp "-OF-" updater))
               (boundp-of-updater-same (symbolicate package-witness boundp-of-updater "-SAME"))
               (boundp-of-updater-diff (symbolicate package-witness boundp-of-updater "-DIFF"))
               (boundp-of-remover (symbolicate package-witness boundp "-OF-" remover))
               (boundp-of-remover-same (symbolicate package-witness boundp-of-remover "-SAME"))
               (boundp-of-remover-diff (symbolicate package-witness boundp-of-remover "-DIFF"))
-              (boundp-when-zp-count (symbolicate package-witness boundp "-WHEN-ZP-" count))
               (boundp-of-keys-set (symbolicate package-witness boundp "-OF-" keys-set))
+              (boundp-when-count-is-zero (symbolicate package-witness boundp "-WHEN-" count "-IS-ZERO"))
 
               (getp-tp (symbolicate package-witness getp "-TP"))
               (getp-rw (symbolicate package-witness getp "-RW"))
@@ -353,8 +423,6 @@
               (remover-when-not-key-recognizer (symbolicate package-witness remover "-WHEN-NOT-" key-recognizer))
               (remover-when-not-recognizer (symbolicate package-witness remover "-WHEN-NOT-" recognizer))
               (remover-of-creator (symbolicate package-witness remover "-OF-" creator))
-              (remover-of-key-fixer (symbolicate package-witness remover "-OF-" key-fixer))
-              (remover-of-fixer (symbolicate package-witness remover "-OF-" fixer))
               (remover-of-updater (symbolicate package-witness remover "-OF-" updater))
               (remover-of-updater-same (symbolicate package-witness remover-of-updater "-SAME"))
               (remover-of-updater-diff (symbolicate package-witness remover-of-updater "-DIFF"))
@@ -362,11 +430,11 @@
               (remover-of-remover (symbolicate package-witness remover "-OF-" remover))
               (remover-of-remover-same (symbolicate package-witness remover-of-remover "-SAME"))
               (remover-of-remover-diff (symbolicate package-witness remover-of-remover "-DIFF"))
+              (remover-when-count-is-zero (symbolicate package-witness remover "-WHEN-" count "-IS-ZERO"))
 
               (count-tp (symbolicate package-witness count "-TP"))
               (count-when-not-recognizer (symbolicate package-witness count "-WHEN-NOT-" recognizer))
               (count-of-creator (symbolicate package-witness count "-OF-" creator))
-              (count-of-fixer (symbolicate package-witness count "-OF-" fixer))
               (count-of-updater (symbolicate package-witness count "-OF-" updater))
               (count-of-updater-when-boundp (symbolicate package-witness count-of-updater "-WHEN-" boundp))
               (count-of-updater-when-not-boundp (symbolicate package-witness count-of-updater "-WHEN-NOT-" boundp))
@@ -375,6 +443,7 @@
               (count-of-remover-when-boundp (symbolicate package-witness count-of-remover "-WHEN-" boundp))
               (count-of-remover-when-not-boundp (symbolicate package-witness count-of-remover "-WHEN-NOT-" boundp))
               (count-of-keys-set (symbolicate package-witness count "-OF-" keys-set))
+              (creator-when-count-is-zero (symbolicate package-witness creator "-WHEN-" count "-IS-ZERO"))
 
               (clear-tp (symbolicate package-witness clear "-TP"))
               (clear-rw (symbolicate package-witness clear "-RW"))
@@ -382,29 +451,9 @@
               (init-tp (symbolicate package-witness init "-TP"))
               (init-rw (symbolicate package-witness init "-RW"))
 
-              (keysp-tp (symbolicate package-witness keysp "-TP"))
-              (keysp-cr (symbolicate package-witness keysp "-CR"))
-              (keysp-def (symbolicate package-witness keysp "-DEF"))
-              (keysp-when-emptyp (symbolicate package-witness keysp "-WHEN-EMPTYP"))
-              (keysp-of-keys-fix (symbolicate package-witness keysp "-OF-" keys-fix))
-              (setp-when-keysp (symbolicate package-witness "SETP-WHEN-" keysp))
-              (key-recognizer-of-head-when-keysp (symbolicate package-witness key-recognizer "-OF-HEAD-WHEN-" keysp))
-              (keysp-of-tail-when-keysp (symbolicate package-witness keysp "-OF-TAIL-WHEN-" keysp))
-              (in-when-keysp (symbolicate package-witness "IN-WHEN-" keysp))
-              (in-when-keysp-split (symbolicate package-witness in-when-keysp "-SPLIT"))
-              (keysp-when-subset (symbolicate package-witness keysp "-WHEN-SUBSET"))
-              (keysp-of-insert (symbolicate package-witness keysp "-OF-INSERT"))
-              (keysp-of-delete (symbolicate package-witness keysp "-OF-DELETE"))
-
-              (keys-fix-tp (symbolicate package-witness keys-fix "-TP"))
-              (keys-fix-when-keysp (symbolicate package-witness keys-fix "-WHEN-" keysp))
-              (keys-fix-when-not-keysp (symbolicate package-witness keys-fix "-WHEN-NOT-" keysp))
-
               (keys-tp (symbolicate package-witness keys "-TP"))
-              (keysp-of-keys (symbolicate package-witness (if key-recognizer keysp "SETP") "-OF-" keys))
               (keys-when-not-recognizer (symbolicate package-witness keys "-WHEN-NOT-" recognizer))
               (keys-of-creator (symbolicate package-witness keys "-OF-" creator))
-              (keys-of-fixer (symbolicate package-witness keys "-OF-" fixer))
               (keys-of-updater (symbolicate package-witness keys "-OF-" updater))
               (keys-of-remover (symbolicate package-witness keys "-OF-" remover))
               (keys-of-keys-set (symbolicate package-witness keys "-OF-" keys-set))
@@ -413,8 +462,6 @@
               (keys-set-when-not-keysp (symbolicate package-witness keys-set "-WHEN-NOT-" (if key-recognizer keysp "SETP")))
               (keys-set-when-not-recognizer (symbolicate package-witness keys-set "-WHEN-NOT-" recognizer))
               (keys-set-of-creator (symbolicate package-witness keys-set "-OF-" creator))
-              (keys-set-of-keys-fix (symbolicate package-witness keys-set "-OF-" (if key-recognizer keys-fix "SFIX")))
-              (keys-set-of-fixer (symbolicate package-witness keys-set "-OF-" fixer))
               (keys-set-of-updater (symbolicate package-witness keys-set "-OF-" updater))
               (keys-set-of-remover (symbolicate package-witness keys-set "-OF-" remover))
               (keys-set-of-keys (symbolicate package-witness keys-set "-OF-" keys))
@@ -429,57 +476,80 @@
               (vals-equal-necc (symbolicate package-witness vals-equal "-NECC"))
               (vals-equal-witness (symbolicate package-witness vals-equal "-WITNESS"))
               (hash-table-equal (symbolicate package-witness hash-table "-EQUAL"))
+              (hash-table-equal-constraints (symbolicate package-witness hash-table-equal "-CONSTRAINTS"))
               (hash-table-equal-fc (symbolicate package-witness hash-table-equal "-FC"))
 
               ;; Epilogue
               (hash-table-theorems (symbolicate package-witness hash-table "-THEOREMS"))
-              (hash-table-definitions (symbolicate package-witness hash-table "-DEFINITIONS"))
               (hash-table-aggressive (symbolicate package-witness hash-table "-AGGRESSIVE"))
               (epilogue
                `((deflabel ,hash-table-end)
-
-                 (deftheory-static ,hash-table-definitions
-                   ',(append
-                      (list contents-recognizer
-                            contents-creator
-                            contents-fixer
-                            contents-accessor
-                            contents-updater
-                            contents-boundp
-                            contents-getp
-                            contents-remover
-                            contents-count
-                            contents-clear
-                            contents-init
-                            hash-table-equal)
-                      (and copyable
-                           key-recognizer
-                           (list keysp
-                                 keys-fix))
-                      (and copyable
-                           (list recognizer
-                                 creator
-                                 fixer
-                                 accessor
-                                 updater
-                                 boundp
-                                 getp
-                                 remover
-                                 count
-                                 clear
-                                 init
-                                 keys
-                                 keys-set))))
 
                  (deftheory-static ,hash-table-theorems
                    (set-difference-theories
                     (set-difference-theories
                      (current-theory ',hash-table-end)
                      (current-theory ',hash-table-begin))
-                    (theory ',hash-table-definitions)))
+                    (union-theories ',(append
+                                       (list contents-recognizer
+                                             contents-creator
+                                             contents-fixer
+                                             equiv
+                                             contents-accessor
+                                             contents-updater
+                                             contents-boundp
+                                             contents-getp
+                                             contents-remover
+                                             contents-count
+                                             contents-clear
+                                             contents-init
+                                             hash-table-equal)
+                                       (and copyable
+                                            (list recognizer
+                                                  creator
+                                                  fixer
+                                                  accessor
+                                                  updater
+                                                  boundp
+                                                  getp
+                                                  remover
+                                                  count
+                                                  clear
+                                                  init
+                                                  keys
+                                                  keys-set))
+                                       (and copyable
+                                            key-recognizer
+                                            (list keysp
+                                                  keys-fix
+                                                  keys-equiv)))
+                                    '(,hash-table-constraints
+                                      ,hash-table-equal-constraints))))
 
                  (deftheory-static ,hash-table-aggressive
                    ',(append
+                      (list accessor-when-not-recognizer
+                            accessor-of-updater
+                            accessor-when-not-boundp
+                            accessor-of-remover
+                            accessor-when-count-is-zero
+                            updater-when-not-recognizer
+                            updater-of-accessor-when-boundp-free
+                            updater-of-accessor
+                            updater-of-updater
+                            boundp-when-not-recognizer
+                            boundp-of-updater
+                            boundp-of-remover
+                            boundp-when-count-is-zero
+                            remover-when-not-recognizer
+                            remover-of-updater
+                            remover-when-not-boundp
+                            remover-of-remover
+                            remover-when-count-is-zero
+                            count-when-not-recognizer
+                            count-of-updater
+                            count-when-boundp
+                            count-of-remover)
                       (and key-recognizer
                            (list accessor-when-not-key-recognizer
                                  updater-when-not-key-recognizer
@@ -494,27 +564,9 @@
                                  keys-set-of-keys-free))
                       (and copyable
                            key-recognizer
-                           (list keys-fix
-                                 in-when-keysp-split))
-                      (list accessor-when-not-recognizer
-                            accessor-of-updater
-                            accessor-when-not-boundp
-                            accessor-of-remover
-                            updater-when-not-recognizer
-                            updater-of-accessor-when-boundp-free
-                            updater-of-accessor
-                            updater-of-updater
-                            boundp-when-not-recognizer
-                            boundp-of-updater
-                            boundp-of-remover
-                            boundp-when-zp-count
-                            remover-when-not-recognizer
-                            remover-of-updater
-                            remover-when-not-boundp
-                            remover-of-remover
-                            count-when-not-recognizer
-                            count-of-updater
-                            count-of-remover)))
+                           (list keysp-when-emptyp
+                                 in-when-keysp-split
+                                 subset-when-keysp))))
 
                  (in-theory
                    (union-theories (current-theory ',hash-table-begin)
@@ -528,14 +580,10 @@
               ;; Functional Instantiation
               (fi-bindings
                (append
-                (list `(lem-hash-table$a::keysp ,(if (and copyable
-                                                          key-recognizer)
-                                                     keysp
-                                                     'set::setp))
-                      `(lem-hash-table$a::keys-fix ,(if (and copyable
-                                                             key-recognizer)
-                                                        keys-fix
-                                                        'set::sfix))
+                (list `(lem-hash-table$a::keysp ,keysp)
+                      `(lem-hash-table$a::keys-fix ,keys-fix)
+                      `(lem-hash-table$a::keys-equiv ,keys-equiv)
+
                       `(lem-hash-table$a::key-recognizer ,(or key-recognizer
                                                               '(lambda (key)
                                                                 t)))
@@ -544,6 +592,8 @@
                       `(lem-hash-table$a::key-fixer ,(or key-fixer
                                                          '(lambda (key)
                                                            key)))
+                      `(lem-hash-table$a::key-equiv ,key-equiv)
+
                       `(lem-hash-table$a::val-recognizer ,(or val-recognizer
                                                               '(lambda (val)
                                                                 t)))
@@ -553,9 +603,14 @@
                       `(lem-hash-table$a::val-fixer ,(or val-fixer
                                                          '(lambda (val)
                                                            val)))
+                      `(lem-hash-table$a::val-equiv ,val-equiv)
+
                       `(lem-hash-table$a::recognizer/unique ,contents-recognizer)
                       `(lem-hash-table$a::creator/unique ,contents-creator)
                       `(lem-hash-table$a::fixer/unique ,contents-fixer)
+                      (if copyable
+                          `(lem-hash-table$a::equiv/copyable ,equiv)
+                          `(lem-hash-table$a::equiv/unique ,equiv))
                       `(lem-hash-table$a::accessor/unique ,contents-accessor)
                       `(lem-hash-table$a::updater/unique ,contents-updater)
                       `(lem-hash-table$a::boundp/unique ,contents-boundp)
@@ -564,6 +619,7 @@
                       `(lem-hash-table$a::count/unique ,contents-count)
                       `(lem-hash-table$a::clear/unique ,contents-clear)
                       `(lem-hash-table$a::init/unique ,contents-init))
+
                 (and copyable
                      (list `(lem-hash-table$a::recognizer/copyable ,recognizer)
                            `(lem-hash-table$a::creator/copyable ,creator)
@@ -578,6 +634,7 @@
                            `(lem-hash-table$a::init/copyable ,init)
                            `(lem-hash-table$a::keys ,keys)
                            `(lem-hash-table$a::keys-set ,keys-set)))))
+
               (fi-bindings-with-contents-skolem
                (list* `(lem-hash-table$a::keys-equal/unique ,keys-equal)
                       `(lem-hash-table$a::keys-equal/unique-witness ,keys-equal-witness)
@@ -600,21 +657,51 @@
 
                   ,@(and key-fixer
                          key-recognizer
+                         (not (eq key-equiv 'equal))
                          `((local
-                             (defthm ,key-fixer-rw
+                             (defthm ,key-recognizer-constraints
+                               (and (booleanp (,key-recognizer ,key))
+                                    (,key-recognizer ,default-key))
+                               :rule-classes
+                               ((:rewrite :corollary
+                                          (booleanp (,key-recognizer ,key))))))
+
+                           (local
+                             (defthm ,key-fixer-constraints
                                (equal (,key-fixer ,key)
                                       (if (,key-recognizer ,key)
                                           ,key
-                                          ,default-key))))))
+                                          ,default-key))))
+
+                           (local
+                             (defthm ,key-equiv-constraints
+                               (equal (,key-equiv ,%key ,key)
+                                      (equal (,key-fixer ,%key)
+                                             (,key-fixer ,key)))))))
 
                   ,@(and val-fixer
                          val-recognizer
+                         (not (eq val-equiv 'equal))
                          `((local
-                             (defthm ,val-fixer-rw
+                             (defthm ,val-recognizer-constraints
+                               (and (booleanp (,val-recognizer ,val))
+                                    (,val-recognizer ,default-val))
+                               :rule-classes
+                               ((:rewrite :corollary
+                                          (booleanp (,val-recognizer ,val))))))
+
+                           (local
+                             (defthm ,val-fixer-constraints
                                (equal (,val-fixer ,val)
                                       (if (,val-recognizer ,val)
                                           ,val
-                                          ,default-val))))))
+                                          ,default-val))))
+
+                           (local
+                             (defthm ,val-equiv-constraints
+                               (equal (,val-equiv ,%val ,val)
+                                      (equal (,val-fixer ,%val)
+                                             (,val-fixer ,val)))))))
 
                   (local
                     (deflabel end-of-prologue))
@@ -637,50 +724,52 @@
                              (in-theory
                                (enable ,@(strip-cars (cdr absstobj-info)))))))
 
-                  (local
-                    (in-theory
-                      (enable acl2::fast-<<-is-<<)))
+                  ,@(and (eq keysp 'set::setp)
+                         `((local
+                             (in-theory
+                               (enable acl2::fast-<<-is-<<)))))
 
                   ,@(and key-recognizer
-                         key-fixer
                          `((local
                              (in-theory
-                               (enable (:e ,key-recognizer)
-                                       (:e ,key-fixer))))))
+                               (enable (:e ,key-recognizer))))))
 
                   ,@(and val-recognizer
-                         val-fixer
                          `((local
                              (in-theory
-                               (enable (:e ,val-recognizer)
-                                       (:e ,val-fixer))))))
+                               (enable (:e ,val-recognizer))))))
 
                   ,@(and copyable
                          key-recognizer
                          `((defun ,keysp (,set)
                              (declare (xargs :guard t))
-                             (if (atom ,set)
-                                 (null ,set)
+                             (if (consp ,set)
                                  (and (,key-recognizer (car ,set))
                                       (or (null (cdr ,set))
                                           (and (consp (cdr ,set))
                                                (<< (car ,set)
                                                    (cadr ,set))
-                                               (,keysp (cdr ,set)))))))
+                                               (,keysp (cdr ,set)))))
+                                 (null ,set)))
 
                            (defun-inline ,keys-fix (,set)
                              (declare (xargs :guard (,keysp ,set)))
                              (mbe :logic (if (,keysp ,set)
                                              ,set
                                              ())
-                                  :exec ,set))))
+                                  :exec ,set))
 
-; If hash-table isn't copyable, then all "CONTENTS"-prefixed symbols refer to
-; their non-prefixed base.
+                           (defun ,keys-equiv (,%set ,set)
+                             (declare (xargs :guard (and (,keysp ,%set)
+                                                         (,keysp ,set))))
+                             (equal (,keys-fix ,%set)
+                                    (,keys-fix ,set)))))
+
+                  ;; If hash-table isn't copyable, then all "CONTENTS"-prefixed
+                  ;; symbols refer to their non-prefixed base.
                   (defun ,contents-recognizer (,contents)
                     (declare (xargs :guard t))
-                    (if (atom ,contents)
-                        (null ,contents)
+                    (if (consp ,contents)
                         (and (consp (car ,contents))
                              ,@(and key-recognizer
                                     `((,key-recognizer (caar ,contents))))
@@ -690,31 +779,24 @@
                                  (and (consp (cdr ,contents))
                                       (consp (cadr ,contents))
                                       (<< (caar ,contents) (caadr ,contents))
-                                      (,contents-recognizer (cdr ,contents)))))))
+                                      (,contents-recognizer (cdr ,contents)))))
+                        (null ,contents)))
 
                   ,@(and copyable
                          `((defun ,recognizer (,hash-table)
                              (declare (xargs :guard t))
                              (and (consp ,hash-table)
-                                  ,(if key-recognizer
-                                       `(,keysp (car ,hash-table))
-                                       `(set::setp (car ,hash-table)))
+                                  (,keysp (car ,hash-table))
                                   (,contents-recognizer (cdr ,hash-table))))))
 
-                  (defun ,contents-creator ()
+                  (defun-nx ,contents-creator ()
                     (declare (xargs :guard t))
                     '())
 
-                  (in-theory
-                    (disable (:e ,contents-creator)))
-
                   ,@(and copyable
-                         `((defun ,creator ()
+                         `((defun-nx ,creator ()
                              (declare (xargs :guard t))
-                             (cons '() (,contents-creator)))
-
-                           (in-theory
-                             (disable (:e ,creator)))))
+                             (cons '() (,contents-creator)))))
 
                   (defun ,contents-fixer (,contents)
                     (declare (xargs :guard (,contents-recognizer ,contents)))
@@ -728,6 +810,12 @@
                              (if (,recognizer ,hash-table)
                                  ,hash-table
                                  (,creator)))))
+
+                  (defun ,equiv (,%hash-table ,hash-table)
+                    (declare (xargs :guard (and (,recognizer ,%hash-table)
+                                                (,recognizer ,hash-table))))
+                    (equal (,fixer ,%hash-table)
+                           (,fixer ,hash-table)))
 
                   (defun ,contents-accessor (,key ,contents)
                     (declare (xargs :guard ,(if key-recognizer
@@ -785,11 +873,9 @@
                         ((endp ,contents)
                          (list (cons ,key ,val)))
                         ((<< ,key (caar ,contents))
-                         (cons (cons ,key ,val)
-                               ,contents))
+                         (cons (cons ,key ,val) ,contents))
                         ((equal ,key (caar ,contents))
-                         (cons (cons ,key ,val)
-                               (cdr ,contents)))
+                         (cons (cons ,key ,val) (cdr ,contents)))
                         (t
                          (cons (car ,contents)
                                (,contents-updater ,key ,val (cdr ,contents)))))))
@@ -904,9 +990,9 @@
                   (defun ,contents-count (,contents)
                     (declare (xargs :guard (,contents-recognizer ,contents)))
                     (let ((,contents (,contents-fixer ,contents)))
-                      (if (endp ,contents)
-                          0
-                          (1+ (,contents-count (cdr ,contents))))))
+                      (if (consp ,contents)
+                          (1+ (,contents-count (cdr ,contents)))
+                          0)))
 
                   ,@(and copyable
                          `((defun ,count (,hash-table)
@@ -962,15 +1048,834 @@
 
                   ,@(and copyable
                          `((defun ,keys-set (,set ,hash-table)
-                             (declare (xargs :guard (and ,(if key-recognizer
-                                                              `(,keysp ,set)
-                                                              `(set::setp ,set))
+                             (declare (xargs :guard (and (,keysp ,set)
                                                          (,recognizer ,hash-table))))
-                             (let ((,set ,(if key-recognizer
-                                              `(,keys-fix ,set)
-                                              `(set::sfix ,set)))
+                             (let ((,set (,keys-fix ,set))
                                    (,hash-table (,fixer ,hash-table)))
                                (cons ,set (cdr ,hash-table))))))
+
+                  (local
+                    ;; This is a hack.
+                    (defthm null-contents
+                      (not (,contents-remover ,key nil))))
+
+                  (defthm ,hash-table-constraints
+                    (and (equal (,contents-recognizer ,contents)
+                                (if (consp ,contents)
+                                    (if (consp (car ,contents))
+                                        ,(cond
+                                           ((and key-recognizer
+                                                 val-recognizer)
+                                            `(if (,key-recognizer (car (car ,contents)))
+                                                 (if (,val-recognizer (cdr (car ,contents)))
+                                                     (if (null (cdr ,contents))
+                                                         (null (cdr ,contents))
+                                                         (if (consp (cdr ,contents))
+                                                             (if (consp (car (cdr ,contents)))
+                                                                 (if (<< (car (car ,contents))
+                                                                         (car (car (cdr ,contents))))
+                                                                     (,contents-recognizer (cdr ,contents))
+                                                                     'nil)
+                                                                 'nil)
+                                                             'nil))
+                                                     'nil)
+                                                 'nil))
+                                           (key-recognizer
+                                            `(if (,key-recognizer (car (car ,contents)))
+                                                 (if (null (cdr ,contents))
+                                                     (null (cdr ,contents))
+                                                     (if (consp (cdr ,contents))
+                                                         (if (consp (car (cdr ,contents)))
+                                                             (if (<< (car (car ,contents))
+                                                                     (car (car (cdr ,contents))))
+                                                                 (,contents-recognizer (cdr ,contents))
+                                                                 'nil)
+                                                             'nil)
+                                                         'nil))
+                                                 'nil))
+                                           (val-recognizer
+                                            `(if (,val-recognizer (cdr (car ,contents)))
+                                                 (if (null (cdr ,contents))
+                                                     (null (cdr ,contents))
+                                                     (if (consp (cdr ,contents))
+                                                         (if (consp (car (cdr ,contents)))
+                                                             (if (<< (car (car ,contents))
+                                                                     (car (car (cdr ,contents))))
+                                                                 (,contents-recognizer (cdr ,contents))
+                                                                 'nil)
+                                                             'nil)
+                                                         'nil))
+                                                 'nil))
+                                           (t
+                                            `(if (null (cdr ,contents))
+                                                 (null (cdr ,contents))
+                                                 (if (consp (cdr ,contents))
+                                                     (if (consp (car (cdr ,contents)))
+                                                         (if (<< (car (car ,contents))
+                                                                 (car (car (cdr ,contents))))
+                                                             (,contents-recognizer (cdr ,contents))
+                                                             'nil)
+                                                         'nil)
+                                                     'nil))))
+                                        'nil)
+                                    (null ,contents)))
+                         (equal (,contents-creator)
+                                'nil)
+                         (equal (,contents-fixer ,contents)
+                                (if (,contents-recognizer ,contents)
+                                    ,contents
+                                    (,contents-creator)))
+                         (equal (,equiv ,%hash-table ,hash-table)
+                                (equal (,fixer ,%hash-table)
+                                       (,fixer ,hash-table)))
+                         (equal (,contents-accessor ,key ,contents)
+                                ((lambda (,key ,contents)
+                                   (if (if (endp ,contents)
+                                           (endp ,contents)
+                                           (<< ,key (car (car ,contents))))
+                                       ,default-val
+                                       (if (equal ,key (car (car ,contents)))
+                                           ,(if val-fixer
+                                                `(,val-fixer (cdr (car ,contents)))
+                                                `(cdr (car ,contents)))
+                                           (,contents-accessor ,key (cdr ,contents)))))
+                                 ,(if key-fixer
+                                      `(,key-fixer ,key)
+                                      key)
+                                 (,contents-fixer ,contents)))
+                         (equal (,contents-updater ,key ,val ,contents)
+                                ((lambda (,key ,val ,contents)
+                                   (if (endp ,contents)
+                                       (cons (cons ,key ,val) 'nil)
+                                       (if (<< ,key (car (car ,contents)))
+                                           (cons (cons ,key ,val) ,contents)
+                                           (if (equal ,key (car (car ,contents)))
+                                               (cons (cons ,key ,val) (cdr ,contents))
+                                               (cons (car ,contents)
+                                                     (,contents-updater ,key ,val (cdr ,contents)))))))
+                                 ,(if key-fixer
+                                      `(,key-fixer ,key)
+                                      key)
+                                 ,(if val-fixer
+                                      `(,val-fixer ,val)
+                                      val)
+                                 (,contents-fixer ,contents)))
+                         (equal (,contents-boundp ,key ,contents)
+                                ((lambda (,key ,contents)
+                                   (if (if (endp ,contents)
+                                           (endp ,contents)
+                                           (<< ,key (car (car ,contents))))
+                                       'nil
+                                       (if (equal ,key (car (car ,contents)))
+                                           't
+                                           (,contents-boundp ,key (cdr ,contents)))))
+                                 ,(if key-fixer
+                                      `(,key-fixer ,key)
+                                      key)
+                                 (,contents-fixer ,contents)))
+                         (equal (,contents-getp ,key ,contents)
+                                ((lambda (,key ,contents)
+                                   (cons (,contents-accessor ,key ,contents)
+                                         (cons (,contents-boundp ,key ,contents)
+                                               'nil)))
+                                 ,(if key-fixer
+                                      `(,key-fixer ,key)
+                                      key)
+                                 (,contents-fixer ,contents)))
+                         (equal (,contents-remover ,key ,contents)
+                                ((lambda (,key ,contents)
+                                   (if (endp ,contents)
+                                       'nil
+                                       (if (<< ,key (car (car ,contents)))
+                                           ,contents
+                                           (if (equal ,key (car (car ,contents)))
+                                               (cdr ,contents)
+                                               (cons (car ,contents)
+                                                     (,contents-remover ,key (cdr ,contents)))))))
+                                 ,(if key-fixer
+                                      `(,key-fixer ,key)
+                                      key)
+                                 (,contents-fixer ,contents)))
+                         (equal (,contents-count ,contents)
+                                ((lambda (,contents)
+                                   (if (consp ,contents)
+                                       (binary-+ '1
+                                                 (,contents-count (cdr ,contents)))
+                                       '0))
+                                 (,contents-fixer ,contents)))
+                         (equal (,contents-clear ,contents)
+                                (,contents-creator))
+                         (equal (,contents-init ht-size rehash-size rehash-threshold ,contents)
+                                (,contents-creator))
+                         ,@(and copyable
+                                `((equal (,keysp ,set)
+                                         (if (consp ,set)
+                                             ,(if key-recognizer
+                                                  `(if (,key-recognizer (car ,set))
+                                                       (if (null (cdr ,set))
+                                                           (null (cdr ,set))
+                                                           (if (consp (cdr ,set))
+                                                               (if (<< (car ,set) (car (cdr ,set)))
+                                                                   (,keysp (cdr ,set))
+                                                                   'nil)
+                                                               'nil))
+                                                       'nil)
+                                                  `(if (null (cdr ,set))
+                                                       (null (cdr ,set))
+                                                       (if (consp (cdr ,set))
+                                                           (if (<< (car ,set) (car (cdr ,set)))
+                                                               (,keysp (cdr ,set))
+                                                               'nil)
+                                                           'nil)))
+                                             (null ,set)))
+                                  (equal (,keys-fix ,set)
+                                         (if (,keysp ,set) ,set 'nil))
+                                  (equal (,keys-equiv ,%set ,set)
+                                         (equal (,keys-fix ,%set) (,keys-fix ,set)))
+                                  (equal (,recognizer hash-table)
+                                         (if (consp hash-table)
+                                             (if (,keysp (car hash-table))
+                                                 (,contents-recognizer (cdr hash-table))
+                                                 'nil)
+                                             'nil))
+                                  (equal (,creator)
+                                         (cons 'nil (,contents-creator)))
+                                  (equal (,fixer hash-table)
+                                         (if (,recognizer hash-table)
+                                             hash-table
+                                             (,creator)))
+                                  (equal (,accessor ,key hash-table)
+                                         ((lambda (,key hash-table)
+                                            (,contents-accessor ,key (cdr hash-table)))
+                                          ,(if key-fixer
+                                               `(,key-fixer ,key)
+                                               key)
+                                          (,fixer hash-table)))
+                                  (equal (,updater ,key ,val hash-table)
+                                         ((lambda (,key ,val hash-table)
+                                            (cons (car hash-table)
+                                                  (,contents-updater ,key ,val (cdr hash-table))))
+                                          ,(if key-fixer
+                                               `(,key-fixer ,key)
+                                               key)
+                                          ,(if val-fixer
+                                               `(,val-fixer ,val)
+                                               val)
+                                          (,fixer hash-table)))
+                                  (equal (,boundp ,key hash-table)
+                                         ((lambda (,key hash-table)
+                                            (,contents-boundp ,key (cdr hash-table)))
+                                          ,(if key-fixer
+                                               `(,key-fixer ,key)
+                                               key)
+                                          (,fixer hash-table)))
+                                  (equal (,getp ,key hash-table)
+                                         ((lambda (,key hash-table)
+                                            (,contents-getp ,key (cdr hash-table)))
+                                          ,(if key-fixer
+                                               `(,key-fixer ,key)
+                                               key)
+                                          (,fixer hash-table)))
+                                  (equal (,remover ,key hash-table)
+                                         ((lambda (,key hash-table)
+                                            (cons (car hash-table)
+                                                  (,contents-remover ,key (cdr hash-table))))
+                                          ,(if key-fixer
+                                               `(,key-fixer ,key)
+                                               key)
+                                          (,fixer hash-table)))
+                                  (equal (,count hash-table)
+                                         ((lambda (hash-table)
+                                            (,contents-count (cdr hash-table)))
+                                          (,fixer hash-table)))
+                                  (equal (,clear hash-table)
+                                         (,creator))
+                                  (equal (,init ht-size
+                                                rehash-size rehash-threshold hash-table)
+                                         (,creator))
+                                  (equal (,keys hash-table)
+                                         ((lambda (hash-table) (car hash-table))
+                                          (,fixer hash-table)))
+                                  (equal (,keys-set ,set hash-table)
+                                         ((lambda (,set hash-table)
+                                            (cons ,set (cdr hash-table)))
+                                          (,keys-fix ,set)
+                                          (,fixer hash-table))))))
+                    :rule-classes
+                    ((:definition :corollary
+                         (equal (,contents-recognizer ,contents)
+                                (if (consp ,contents)
+                                    (if (consp (car ,contents))
+                                        ,(cond
+                                           ((and key-recognizer
+                                                 val-recognizer)
+                                            `(if (,key-recognizer (car (car ,contents)))
+                                                 (if (,val-recognizer (cdr (car ,contents)))
+                                                     (if (null (cdr ,contents))
+                                                         (null (cdr ,contents))
+                                                         (if (consp (cdr ,contents))
+                                                             (if (consp (car (cdr ,contents)))
+                                                                 (if (<< (car (car ,contents))
+                                                                         (car (car (cdr ,contents))))
+                                                                     (,contents-recognizer (cdr ,contents))
+                                                                     'nil)
+                                                                 'nil)
+                                                             'nil))
+                                                     'nil)
+                                                 'nil))
+                                           (key-recognizer
+                                            `(if (,key-recognizer (car (car ,contents)))
+                                                 (if (null (cdr ,contents))
+                                                     (null (cdr ,contents))
+                                                     (if (consp (cdr ,contents))
+                                                         (if (consp (car (cdr ,contents)))
+                                                             (if (<< (car (car ,contents))
+                                                                     (car (car (cdr ,contents))))
+                                                                 (,contents-recognizer (cdr ,contents))
+                                                                 'nil)
+                                                             'nil)
+                                                         'nil))
+                                                 'nil))
+                                           (val-recognizer
+                                            `(if (,val-recognizer (cdr (car ,contents)))
+                                                 (if (null (cdr ,contents))
+                                                     (null (cdr ,contents))
+                                                     (if (consp (cdr ,contents))
+                                                         (if (consp (car (cdr ,contents)))
+                                                             (if (<< (car (car ,contents))
+                                                                     (car (car (cdr ,contents))))
+                                                                 (,contents-recognizer (cdr ,contents))
+                                                                 'nil)
+                                                             'nil)
+                                                         'nil))
+                                                 'nil))
+                                           (t
+                                            `(if (null (cdr ,contents))
+                                                 (null (cdr ,contents))
+                                                 (if (consp (cdr ,contents))
+                                                     (if (consp (car (cdr ,contents)))
+                                                         (if (<< (car (car ,contents))
+                                                                 (car (car (cdr ,contents))))
+                                                             (,contents-recognizer (cdr ,contents))
+                                                             'nil)
+                                                         'nil)
+                                                     'nil))))
+                                        'nil)
+                                    (null ,contents))))
+                     (:definition :corollary
+                         (equal (,contents-creator)
+                                'nil))
+                     (:definition :corollary
+                         (equal (,contents-fixer ,contents)
+                                (if (,contents-recognizer ,contents)
+                                    ,contents
+                                    (,contents-creator))))
+                     (:definition :corollary
+                         (equal (,equiv ,%hash-table ,hash-table)
+                                (equal (,fixer ,%hash-table)
+                                       (,fixer ,hash-table))))
+                     (:definition :corollary
+                         (equal (,contents-accessor ,key ,contents)
+                                ((lambda (,key ,contents)
+                                   (if (if (endp ,contents)
+                                           (endp ,contents)
+                                           (<< ,key (car (car ,contents))))
+                                       ,default-val
+                                       (if (equal ,key (car (car ,contents)))
+                                           ,(if val-fixer
+                                                `(,val-fixer (cdr (car ,contents)))
+                                                `(cdr (car ,contents)))
+                                           (,contents-accessor ,key (cdr ,contents)))))
+                                 ,(if key-fixer
+                                      `(,key-fixer ,key)
+                                      key)
+                                 (,contents-fixer ,contents))))
+                     (:definition :corollary
+                         (equal (,contents-updater ,key ,val ,contents)
+                                ((lambda (,key ,val ,contents)
+                                   (if (endp ,contents)
+                                       (cons (cons ,key ,val) 'nil)
+                                       (if (<< ,key (car (car ,contents)))
+                                           (cons (cons ,key ,val) ,contents)
+                                           (if (equal ,key (car (car ,contents)))
+                                               (cons (cons ,key ,val) (cdr ,contents))
+                                               (cons (car ,contents)
+                                                     (,contents-updater ,key ,val (cdr ,contents)))))))
+                                 ,(if key-fixer
+                                      `(,key-fixer ,key)
+                                      key)
+                                 ,(if val-fixer
+                                      `(,val-fixer ,val)
+                                      val)
+                                 (,contents-fixer ,contents))))
+                     (:definition :corollary
+                         (equal (,contents-boundp ,key ,contents)
+                                ((lambda (,key ,contents)
+                                   (if (if (endp ,contents)
+                                           (endp ,contents)
+                                           (<< ,key (car (car ,contents))))
+                                       'nil
+                                       (if (equal ,key (car (car ,contents)))
+                                           't
+                                           (,contents-boundp ,key (cdr ,contents)))))
+                                 ,(if key-fixer
+                                      `(,key-fixer ,key)
+                                      key)
+                                 (,contents-fixer ,contents))))
+                     (:definition :corollary
+                         (equal (,contents-getp ,key ,contents)
+                                ((lambda (,key ,contents)
+                                   (cons (,contents-accessor ,key ,contents)
+                                         (cons (,contents-boundp ,key ,contents)
+                                               'nil)))
+                                 ,(if key-fixer
+                                      `(,key-fixer ,key)
+                                      key)
+                                 (,contents-fixer ,contents))))
+                     (:definition :corollary
+                         (equal (,contents-remover ,key ,contents)
+                                ((lambda (,key ,contents)
+                                   (if (endp ,contents)
+                                       'nil
+                                       (if (<< ,key (car (car ,contents)))
+                                           ,contents
+                                           (if (equal ,key (car (car ,contents)))
+                                               (cdr ,contents)
+                                               (cons (car ,contents)
+                                                     (,contents-remover ,key (cdr ,contents)))))))
+                                 ,(if key-fixer
+                                      `(,key-fixer ,key)
+                                      key)
+                                 (,contents-fixer ,contents))))
+                     (:definition :corollary
+                         (equal (,contents-count ,contents)
+                                ((lambda (,contents)
+                                   (if (consp ,contents)
+                                       (binary-+ '1
+                                                 (,contents-count (cdr ,contents)))
+                                       '0))
+                                 (,contents-fixer ,contents))))
+                     (:definition :corollary
+                         (equal (,contents-clear ,contents)
+                                (,contents-creator)))
+                     (:definition :corollary
+                         (equal (,contents-init ht-size rehash-size rehash-threshold ,contents)
+                                (,contents-creator)))
+                     ,@(and copyable
+                            `((:definition :corollary
+                                  (equal (,keysp ,set)
+                                         (if (consp ,set)
+                                             ,(if key-recognizer
+                                                  `(if (,key-recognizer (car ,set))
+                                                       (if (null (cdr ,set))
+                                                           (null (cdr ,set))
+                                                           (if (consp (cdr ,set))
+                                                               (if (<< (car ,set) (car (cdr ,set)))
+                                                                   (,keysp (cdr ,set))
+                                                                   'nil)
+                                                               'nil))
+                                                       'nil)
+                                                  `(if (null (cdr ,set))
+                                                       (null (cdr ,set))
+                                                       (if (consp (cdr ,set))
+                                                           (if (<< (car ,set) (car (cdr ,set)))
+                                                               (,keysp (cdr ,set))
+                                                               'nil)
+                                                           'nil)))
+                                             (null ,set))))
+                              (:definition :corollary
+                                  (equal (,keys-fix ,set)
+                                         (if (,keysp ,set) ,set 'nil)))
+                              (:definition :corollary
+                                  (equal (,keys-equiv ,%set ,set)
+                                         (equal (,keys-fix ,%set) (,keys-fix ,set))))
+                              (:definition :corollary
+                                  (equal (,recognizer hash-table)
+                                         (if (consp hash-table)
+                                             (if (,keysp (car hash-table))
+                                                 (,contents-recognizer (cdr hash-table))
+                                                 'nil)
+                                             'nil)))
+                              (:definition :corollary
+                                  (equal (,creator)
+                                         (cons 'nil (,contents-creator))))
+                              (:definition :corollary
+                                  (equal (,fixer hash-table)
+                                         (if (,recognizer hash-table)
+                                             hash-table
+                                             (,creator))))
+                              (:definition :corollary
+                                  (equal (,accessor ,key hash-table)
+                                         ((lambda (,key hash-table)
+                                            (,contents-accessor ,key (cdr hash-table)))
+                                          ,(if key-fixer
+                                               `(,key-fixer ,key)
+                                               key)
+                                          (,fixer hash-table))))
+                              (:definition :corollary
+                                  (equal (,updater ,key ,val hash-table)
+                                         ((lambda (,key ,val hash-table)
+                                            (cons (car hash-table)
+                                                  (,contents-updater ,key ,val (cdr hash-table))))
+                                          ,(if key-fixer
+                                               `(,key-fixer ,key)
+                                               key)
+                                          ,(if val-fixer
+                                               `(,val-fixer ,val)
+                                               val)
+                                          (,fixer hash-table))))
+                              (:definition :corollary
+                                  (equal (,boundp ,key hash-table)
+                                         ((lambda (,key hash-table)
+                                            (,contents-boundp ,key (cdr hash-table)))
+                                          ,(if key-fixer
+                                               `(,key-fixer ,key)
+                                               key)
+                                          (,fixer hash-table))))
+                              (:definition :corollary
+                                  (equal (,getp ,key hash-table)
+                                         ((lambda (,key hash-table)
+                                            (,contents-getp ,key (cdr hash-table)))
+                                          ,(if key-fixer
+                                               `(,key-fixer ,key)
+                                               key)
+                                          (,fixer hash-table))))
+                              (:definition :corollary
+                                  (equal (,remover ,key hash-table)
+                                         ((lambda (,key hash-table)
+                                            (cons (car hash-table)
+                                                  (,contents-remover ,key (cdr hash-table))))
+                                          ,(if key-fixer
+                                               `(,key-fixer ,key)
+                                               key)
+                                          (,fixer hash-table))))
+                              (:definition :corollary
+                                  (equal (,count hash-table)
+                                         ((lambda (hash-table)
+                                            (,contents-count (cdr hash-table)))
+                                          (,fixer hash-table))))
+                              (:definition :corollary
+                                  (equal (,clear hash-table)
+                                         (,creator)))
+                              (:definition :corollary
+                                  (equal (,init ht-size
+                                                rehash-size rehash-threshold hash-table)
+                                         (,creator)))
+                              (:definition :corollary
+                                  (equal (,keys hash-table)
+                                         ((lambda (hash-table) (car hash-table))
+                                          (,fixer hash-table))))
+                              (:definition :corollary
+                                  (equal (,keys-set ,set hash-table)
+                                         ((lambda (,set hash-table)
+                                            (cons ,set (cdr hash-table)))
+                                          (,keys-fix ,set)
+                                          (,fixer hash-table)))))))
+                    :hints
+                    (("Goal"
+                      :do-not-induct t
+                      ,@(and (eq keysp 'set::setp)
+                             `(:in-theory (enable set::setp
+                                                  set::sfix
+                                                  set::equiv
+                                                  set::emptyp))))))
+
+                  (local
+                    (in-theory
+                      (disable ,@(and copyable
+                                      key-recognizer
+                                      (list keysp
+                                            keys-fix
+                                            keys-equiv))
+                               ,contents-recognizer
+                               ,contents-creator
+                               ,contents-fixer
+                               ,equiv
+                               ,contents-accessor
+                               ,contents-updater
+                               ,contents-boundp
+                               ,contents-getp
+                               ,contents-remover
+                               ,contents-count
+                               ,contents-clear
+                               ,contents-init
+                               ,@(and copyable
+                                      (list keys
+                                            keys-set
+                                            recognizer
+                                            creator
+                                            fixer
+                                            accessor
+                                            updater
+                                            boundp
+                                            getp
+                                            remover
+                                            count
+                                            clear
+                                            init)))))
+
+                  ;; `KEYSP'
+                  ,@(and copyable
+                         key-recognizer
+                         `((defthm ,keysp-tp
+                             (booleanp (,keysp ,set))
+                             :rule-classes :type-prescription
+                             :hints
+                             (("Goal"
+                               :by (:functional-instance
+                                    lem-hash-table$a::keysp-tp
+                                    ,@fi-bindings))))
+
+                           (defthm ,keysp-cr
+                             (implies (,keysp ,set)
+                                      (true-listp ,set))
+                             :rule-classes :compound-recognizer
+                             :hints
+                             (("Goal"
+                               :by (:functional-instance
+                                    lem-hash-table$a::keysp-cr
+                                    ,@fi-bindings))))
+
+                           (defthmd ,keysp-def
+                             (equal (,keysp ,set)
+                                    (and (set::setp ,set)
+                                         (or (set::emptyp ,set)
+                                             (and (,key-recognizer (set::head ,set))
+                                                  (,keysp (set::tail ,set))))))
+                             :rule-classes
+                             ((:definition :controller-alist ((,keysp t))))
+                             :hints
+                             (("Goal"
+                               :by (:functional-instance
+                                    lem-hash-table$a::keysp-def
+                                    ,@fi-bindings))))
+
+                           (defthm ,setp-when-keysp
+                             (implies (,keysp ,set)
+                                      (set::setp ,set))
+                             :hints
+                             (("Goal"
+                               :by (:functional-instance
+                                    lem-hash-table$a::setp-when-keysp
+                                    ,@fi-bindings))))
+
+                           (defthmd ,keysp-when-emptyp
+                             (implies (set::emptyp ,set)
+                                      (equal (,keysp ,set)
+                                             (set::setp ,set)))
+                             :hints
+                             (("Goal"
+                               :by (:functional-instance
+                                    lem-hash-table$a::keysp-when-emptyp
+                                    ,@fi-bindings))))
+
+                           (defthm ,keysp-of-keys-fix
+                             (,keysp (,keys-fix ,set))
+                             :hints
+                             (("Goal"
+                               :by (:functional-instance
+                                    lem-hash-table$a::keysp-of-keys-fix
+                                    ,@fi-bindings))))
+
+                           (defthm ,keysp-of-keys
+                             (,keysp (,keys ,hash-table))
+                             :hints
+                             (("Goal"
+                               :by (:functional-instance
+                                    lem-hash-table$a::keysp-of-keys
+                                    ,@fi-bindings))))
+
+                           (defthm ,keysp-of-sfix
+                             (equal (,keysp (set::sfix set))
+                                    (or (set::emptyp set)
+                                        (,keysp set)))
+                             :hints
+                             (("Goal"
+                               :by (:functional-instance
+                                    lem-hash-table$a::keysp-of-sfix
+                                    ,@fi-bindings))))
+
+                           (defthm ,key-recognizer-of-head-when-keysp
+                             (implies (and (not (set::emptyp ,set))
+                                           (,keysp ,set))
+                                      (,key-recognizer (set::head ,set)))
+                             :hints
+                             (("Goal"
+                               :by (:functional-instance
+                                    lem-hash-table$a::key-recognizer-of-head-when-keysp
+                                    ,@fi-bindings))))
+
+                           (defthm ,keysp-of-tail-when-keysp
+                             (implies (and (not (set::emptyp ,set))
+                                           (,keysp ,set))
+                                      (,keysp (set::tail ,set)))
+                             :hints
+                             (("Goal"
+                               :by (:functional-instance
+                                    lem-hash-table$a::keysp-of-tail-when-keysp
+                                    ,@fi-bindings))))
+
+
+                           (defthm ,keysp-of-insert
+                             (equal (,keysp (set::insert key set))
+                                    (and (,key-recognizer key)
+                                         (or (set::emptyp set)
+                                             (,keysp set))))
+                             :hints
+                             (("Goal"
+                               :by (:functional-instance
+                                    lem-hash-table$a::keysp-of-insert
+                                    ,@fi-bindings))))
+
+                           (defthmd ,in-when-keysp-split
+                             (implies (and (,keysp ,set)
+                                           (not (,key-recognizer ,key)))
+                                      (not (set::in ,key ,set)))
+                             :rule-classes
+                             ((:rewrite :corollary
+                                        (implies (and (,keysp ,set)
+                                                      (not (case-split (,key-recognizer ,key))))
+                                                 (not (set::in ,key ,set)))))
+                             :hints
+                             (("Goal"
+                               :by (:functional-instance
+                                    lem-hash-table$a::in-when-keysp
+                                    ,@fi-bindings))))
+
+                           (defthm ,in-when-keysp
+                             (implies (and (,keysp ,set)
+                                           (not (,key-recognizer ,key)))
+                                      (not (set::in ,key ,set)))
+                             :hints
+                             (("Goal"
+                               :by (:functional-instance
+                                    lem-hash-table$a::in-when-keysp
+                                    ,@fi-bindings))))
+
+                           (defthmd ,subset-when-keysp
+                             (implies (and (not (,keysp ,%set))
+                                           (,keysp ,set))
+                                      (equal (set::subset ,%set ,set)
+                                             (set::emptyp ,%set)))
+                             :hints
+                             (("Goal"
+                               :by (:functional-instance
+                                    lem-hash-table$a::subset-when-keysp
+                                    ,@fi-bindings))))
+
+                           (defthm ,keysp-of-delete
+                             (implies (,keysp ,set)
+                                      (,keysp (set::delete ,key ,set)))
+                             :hints
+                             (("Goal"
+                               :by (:functional-instance
+                                    lem-hash-table$a::keysp-of-delete
+                                    ,@fi-bindings))))
+
+                           (defthm ,keysp-of-union
+                             (equal (,keysp (set::union ,%set ,set))
+                                    (and (or (set::emptyp ,%set)
+                                             (,keysp ,%set))
+                                         (or (set::emptyp ,set)
+                                             (,keysp ,set))))
+                             :hints
+                             (("Goal"
+                               :by (:functional-instance
+                                    lem-hash-table$a::keysp-of-union
+                                    ,@fi-bindings))))
+
+                           (defthm ,keysp-of-intersect
+                             (implies (or (,keysp ,%set)
+                                          (,keysp ,set))
+                                      (,keysp (set::intersect ,%set ,set)))
+                             :hints
+                             (("Goal"
+                               :by (:functional-instance
+                                    lem-hash-table$a::keysp-of-intersect
+                                    ,@fi-bindings))))
+
+                           (defthm ,keysp-of-difference
+                             (implies (,keysp ,%set)
+                                      (,keysp (set::difference ,%set ,set)))
+                             :hints
+                             (("Goal"
+                               :by (:functional-instance
+                                    lem-hash-table$a::keysp-of-difference
+                                    ,@fi-bindings))))))
+
+                  ;; `KEYS-FIX'
+                  ,@(and copyable
+                         key-recognizer
+                         `((defthm ,keys-fix-tp
+                             (true-listp (,keys-fix ,set))
+                             :rule-classes :type-prescription
+                             :hints
+                             (("Goal"
+                               :by (:functional-instance
+                                    lem-hash-table$a::keys-fix-tp
+                                    ,@fi-bindings))))
+
+                           (defthm ,keys-fix-when-keysp
+                             (implies (,keysp ,set)
+                                      (equal (,keys-fix ,set)
+                                             ,set))
+                             :hints
+                             (("Goal"
+                               :by (:functional-instance
+                                    lem-hash-table$a::keys-fix-when-keysp
+                                    ,@fi-bindings))))
+
+                           (defthm ,keys-fix-when-not-keysp
+                             (implies (not (,keysp ,set))
+                                      (not (,keys-fix ,set)))
+                             :hints
+                             (("Goal"
+                               :by (:functional-instance
+                                    lem-hash-table$a::keys-fix-when-not-keysp
+                                    ,@fi-bindings))))))
+
+                  ;; `KEYS-EQUIV'
+                  ,@(and copyable
+                         key-recognizer
+                         `((defthm ,keys-equiv-tp
+                             (booleanp (,keys-equiv ,%set ,set))
+                             :rule-classes :type-prescription
+                             :hints
+                             (("Goal"
+                               :by (:functional-instance
+                                    lem-hash-table$a::keys-equiv-tp
+                                    ,@fi-bindings))))
+
+                           (defequiv ,keys-equiv
+                             :hints
+                             (("Goal"
+                               :by (:functional-instance
+                                    lem-hash-table$a::keys-equiv-is-an-equivalence
+                                    ,@fi-bindings))))
+
+                           (defcong ,keys-equiv equal (,keys-fix ,set) 1
+                             :hints
+                             (("Goal"
+                               :by (:functional-instance
+                                    lem-hash-table$a::keys-equiv-implies-equal-keys-fix-1
+                                    ,@fi-bindings))))
+
+                           (defthm ,keys-fix-mod-keys-equiv
+                             (,keys-equiv (,keys-fix ,set) ,set)
+                             :hints
+                             (("Goal"
+                               :by (:functional-instance
+                                    lem-hash-table$a::keys-fix-mod-keys-equiv
+                                    ,@fi-bindings))))
+
+                           (defthm ,keys-equiv-when-not-keysp
+                             (implies (not (,keysp ,set))
+                                      (,keys-equiv ,set ()))
+                             :hints
+                             (("Goal"
+                               :by (:functional-instance
+                                    lem-hash-table$a::keys-equiv-when-not-keysp
+                                    ,@fi-bindings))))))
 
                   ;; `RECOGNIZER'
                   (defthm ,recognizer-tp
@@ -978,10 +1883,6 @@
                     :rule-classes :type-prescription
                     :hints
                     (("Goal"
-                      ,@(and (not key-recognizer)
-                             `(:in-theory (enable set::setp
-                                                  set::sfix
-                                                  set::emptyp)))
                       :by (:functional-instance
                            ,(if copyable
                                 'lem-hash-table$a::recognizer/copyable-tp
@@ -1048,10 +1949,6 @@
                              (,recognizer (,keys-set ,set ,hash-table))
                              :hints
                              (("Goal"
-                               ,@(and (not key-recognizer)
-                                      `(:in-theory (enable set::setp
-                                                           set::sfix
-                                                           set::emptyp)))
                                :by (:functional-instance
                                     lem-hash-table$a::recognizer/copyable-of-keys-set
                                     ,@fi-bindings))))))
@@ -1095,6 +1992,57 @@
                                 'lem-hash-table$a::fixer/unique-when-not-recognizer/unique)
                            ,@fi-bindings))))
 
+                  ;; `EQUIV'
+                  (defthm ,equiv-tp
+                    (booleanp (,equiv ,%hash-table ,hash-table))
+                    :rule-classes :type-prescription
+                    :hints
+                    (("Goal"
+                      :by (:functional-instance
+                           ,(if copyable
+                                'lem-hash-table$a::equiv/copyable-tp
+                                'lem-hash-table$a::equiv/unique-tp)
+                           ,@fi-bindings))))
+
+                  (defequiv ,equiv
+                    :hints
+                    (("Goal"
+                      :by (:functional-instance
+                           ,(if copyable
+                                'lem-hash-table$a::equiv/copyable-is-an-equivalence
+                                'lem-hash-table$a::equiv/unique-is-an-equivalence)
+                           ,@fi-bindings))))
+
+                  (defcong ,equiv equal (,fixer ,hash-table) 1
+                    :hints
+                    (("Goal"
+                      :by (:functional-instance
+                           ,(if copyable
+                                'lem-hash-table$a::equiv/copyable-implies-equal-fixer/copyable-1
+                                'lem-hash-table$a::equiv/unique-implies-equal-fixer/unique-1)
+                           ,@fi-bindings))))
+
+                  (defthm ,fixer-mod-equiv
+                    (,equiv (,fixer ,hash-table) ,hash-table)
+                    :hints
+                    (("Goal"
+                      :by (:functional-instance
+                           ,(if copyable
+                                'lem-hash-table$a::fixer/copyable-mod-equiv/copyable
+                                'lem-hash-table$a::fixer/unique-mod-equiv/unique)
+                           ,@fi-bindings))))
+
+                  (defthm ,equiv-when-not-recognizer
+                    (implies (not (,recognizer ,hash-table))
+                             (,equiv ,hash-table (,creator)))
+                    :hints
+                    (("Goal"
+                      :by (:functional-instance
+                           ,(if copyable
+                                'lem-hash-table$a::equiv/copyable-when-not-recognizer/copyable
+                                'lem-hash-table$a::equiv/unique-when-not-recognizer/unique)
+                           ,@fi-bindings))))
+
                   ;; `ACCESSOR'
                   ,@(and val-recognizer
                          `((defthm ,val-recognizer-of-accessor
@@ -1104,13 +2052,32 @@
                               :type-prescription)
                              :hints
                              (("Goal"
-                               ,@(and val-creator
-                                      `(:in-theory (enable (:e ,val-creator))))
                                :by (:functional-instance
                                     ,(if copyable
                                          'lem-hash-table$a::val-recognizer-of-accessor/copyable
                                          'lem-hash-table$a::val-recognizer-of-accessor/unique)
                                     ,@fi-bindings))))))
+
+                  ,@(and key-recognizer
+                         key-fixer
+                         (not (eq key-equiv 'equal))
+                         `((defcong ,key-equiv equal (,accessor ,key ,hash-table) 1
+                             :hints
+                             (("Goal"
+                               :by (:functional-instance
+                                    ,(if copyable
+                                         'lem-hash-table$a::key-equiv-implies-equal-accessor/copyable-1
+                                         'lem-hash-table$a::key-equiv-implies-equal-accessor/unique-1)
+                                    ,@fi-bindings))))))
+
+                  (defcong ,equiv equal (,accessor ,key ,hash-table) 2
+                    :hints
+                    (("Goal"
+                      :by (:functional-instance
+                           ,(if copyable
+                                'lem-hash-table$a::equiv/copyable-implies-equal-accessor/copyable-2
+                                'lem-hash-table$a::equiv/unique-implies-equal-accessor/unique-2)
+                           ,@fi-bindings))))
 
                   ,@(and key-recognizer
                          `((defthmd ,accessor-when-not-key-recognizer
@@ -1148,41 +2115,23 @@
                                 'lem-hash-table$a::accessor/unique-of-creator/unique)
                            ,@fi-bindings))))
 
-                  ,@(and key-fixer
-                         `((defthm ,accessor-of-key-fixer
-                             (equal (,accessor (,key-fixer ,key) ,hash-table)
-                                    (,accessor ,key ,hash-table))
-                             :hints
-                             (("Goal"
-                               :by (:functional-instance
-                                    ,(if copyable
-                                         'lem-hash-table$a::accessor/copyable-of-key-fixer
-                                         'lem-hash-table$a::accessor/unique-of-key-fixer)
-                                    ,@fi-bindings))))))
-
-                  (defthm ,accessor-of-fixer
-                    (equal (,accessor ,key (,fixer ,hash-table))
-                           (,accessor ,key ,hash-table))
-                    :hints
-                    (("Goal"
-                      :by (:functional-instance
-                           ,(if copyable
-                                'lem-hash-table$a::accessor/copyable-of-fixer/copyable
-                                'lem-hash-table$a::accessor/unique-of-fixer/unique)
-                           ,@fi-bindings))))
-
                   (defthmd ,accessor-of-updater
                     (equal (,accessor ,%key (,updater ,key ,val ,hash-table))
-                           (if (equal ,(if key-fixer
-                                           `(,key-fixer ,%key)
-                                           %key)
-                                      ,(if key-fixer
-                                           `(,key-fixer ,key)
-                                           key))
+                           (if (,key-equiv ,%key ,key)
                                ,(if val-fixer
                                     `(,val-fixer ,val)
                                     val)
                                (,accessor ,%key ,hash-table)))
+                    :rule-classes
+                    ((:rewrite :corollary
+                               (equal (,accessor ,%key (,updater ,key ,val ,hash-table))
+                                      (if (,key-equiv ,%key ,(if (eq key-equiv 'equal)
+                                                                 key
+                                                                 `(double-rewrite ,key)))
+                                          ,(if val-fixer
+                                               `(,val-fixer (double-rewrite ,val))
+                                               val)
+                                          (,accessor ,%key (double-rewrite ,hash-table))))))
                     :hints
                     (("Goal"
                       :by (:functional-instance
@@ -1192,16 +2141,20 @@
                            ,@fi-bindings))))
 
                   (defthm ,accessor-of-updater-same
-                    (implies (equal ,(if key-fixer
-                                         `(,key-fixer ,%key)
-                                         %key)
-                                    ,(if key-fixer
-                                         `(,key-fixer ,key)
-                                         key))
+                    (implies (,key-equiv ,%key ,key)
                              (equal (,accessor ,%key (,updater ,key ,val ,hash-table))
                                     ,(if val-fixer
                                          `(,val-fixer ,val)
                                          val)))
+                    :rule-classes
+                    ((:rewrite :corollary
+                               (implies (,key-equiv ,%key ,(if (eq key-equiv 'equal)
+                                                               key
+                                                               `(double-rewrite ,key)))
+                                        (equal (,accessor ,%key (,updater ,key ,val ,hash-table))
+                                               ,(if val-fixer
+                                                    `(,val-fixer (double-rewrite ,val))
+                                                    val)))))
                     :hints
                     (("Goal"
                       :by (:functional-instance
@@ -1211,14 +2164,16 @@
                            ,@fi-bindings))))
 
                   (defthm ,accessor-of-updater-diff
-                    (implies (not (equal ,(if key-fixer
-                                              `(,key-fixer ,%key)
-                                              %key)
-                                         ,(if key-fixer
-                                              `(,key-fixer ,key)
-                                              key)))
+                    (implies (not (,key-equiv ,%key ,key))
                              (equal (,accessor ,%key (,updater ,key ,val ,hash-table))
                                     (,accessor ,%key ,hash-table)))
+                    :rule-classes
+                    ((:rewrite :corollary
+                               (implies (not (,key-equiv ,%key ,(if (eq key-equiv 'equal)
+                                                                    key
+                                                                    `(double-rewrite ,key))))
+                                        (equal (,accessor ,%key (,updater ,key ,val ,hash-table))
+                                               (,accessor ,%key (double-rewrite ,hash-table))))))
                     :hints
                     (("Goal"
                       :by (:functional-instance
@@ -1227,7 +2182,7 @@
                                 'lem-hash-table$a::accessor/unique-of-updater/unique-diff)
                            ,@fi-bindings))))
 
-                  (defthmd , accessor-when-not-boundp
+                  (defthmd ,accessor-when-not-boundp
                     (implies (not (,boundp ,key ,hash-table))
                              (equal (,accessor ,key ,hash-table)
                                     ,default-val))
@@ -1241,14 +2196,17 @@
 
                   (defthmd ,accessor-of-remover
                     (equal (,accessor ,%key (,remover ,key ,hash-table))
-                           (if (equal ,(if key-fixer
-                                           `(,key-fixer ,%key)
-                                           %key)
-                                      ,(if key-fixer
-                                           `(,key-fixer ,key)
-                                           key))
+                           (if (,key-equiv ,%key ,key)
                                ,default-val
                                (,accessor ,%key ,hash-table)))
+                    :rule-classes
+                    ((:rewrite :corollary
+                               (equal (,accessor ,%key (,remover ,key ,hash-table))
+                                      (if (,key-equiv ,%key ,(if (eq key-equiv 'equal)
+                                                                 key
+                                                                 `(double-rewrite ,key)))
+                                          ,default-val
+                                          (,accessor ,%key (double-rewrite ,hash-table))))))
                     :hints
                     (("Goal"
                       :by (:functional-instance
@@ -1258,14 +2216,16 @@
                            ,@fi-bindings))))
 
                   (defthm ,accessor-of-remover-same
-                    (implies (equal ,(if key-fixer
-                                         `(,key-fixer ,%key)
-                                         %key)
-                                    ,(if key-fixer
-                                         `(,key-fixer ,key)
-                                         key))
+                    (implies (,key-equiv ,%key ,key)
                              (equal (,accessor ,%key (,remover ,key ,hash-table))
                                     ,default-val))
+                    :rule-classes
+                    ((:rewrite :corollary
+                               (implies (,key-equiv ,%key ,(if (eq key-equiv 'equal)
+                                                               key
+                                                               `(double-rewrite ,key)))
+                                        (equal (,accessor ,%key (,remover ,key ,hash-table))
+                                               ,default-val))))
                     :hints
                     (("Goal"
                       :by (:functional-instance
@@ -1275,14 +2235,16 @@
                            ,@fi-bindings))))
 
                   (defthm ,accessor-of-remover-diff
-                    (implies (not (equal ,(if key-fixer
-                                              `(,key-fixer ,%key)
-                                              %key)
-                                         ,(if key-fixer
-                                              `(,key-fixer ,key)
-                                              key)))
+                    (implies (not (,key-equiv ,%key ,key))
                              (equal (,accessor ,%key (,remover ,key ,hash-table))
                                     (,accessor ,%key ,hash-table)))
+                    :rule-classes
+                    ((:rewrite :corollary
+                               (implies (not (,key-equiv ,%key ,(if (eq key-equiv 'equal)
+                                                                    key
+                                                                    `(double-rewrite ,key))))
+                                        (equal (,accessor ,%key (,remover ,key ,hash-table))
+                                               (,accessor ,%key (double-rewrite ,hash-table))))))
                     :hints
                     (("Goal"
                       :by (:functional-instance
@@ -1295,11 +2257,27 @@
                          `((defthm ,accessor-of-keys-set
                              (equal (,accessor ,key (,keys-set ,set ,hash-table))
                                     (,accessor ,key ,hash-table))
+                             :rule-classes
+                             ((:rewrite :corollary
+                                        (equal (,accessor ,key (,keys-set ,set ,hash-table))
+                                               (,accessor ,key (double-rewrite ,hash-table)))))
                              :hints
                              (("Goal"
                                :by (:functional-instance
                                     lem-hash-table$a::accessor/copyable-of-keys-set
                                     ,@fi-bindings))))))
+
+                  (defthmd ,accessor-when-count-is-zero
+                    (implies (equal (,count ,hash-table) 0)
+                             (equal (,accessor ,key ,hash-table)
+                                    ,default-val))
+                    :hints
+                    (("Goal"
+                      :by (:functional-instance
+                           ,(if copyable
+                                'lem-hash-table$a::accessor/copyable-when-count/copyable-is-zero
+                                'lem-hash-table$a::accessor/unique-when-count/unique-is-zero)
+                           ,@fi-bindings))))
 
                   ;; `UPDATER'
                   (defthm ,updater-tp
@@ -1314,6 +2292,39 @@
                            ,(if copyable
                                 'lem-hash-table$a::updater/copyable-tp
                                 'lem-hash-table$a::updater/unique-tp)
+                           ,@fi-bindings))))
+
+                  ,@(and key-recognizer
+                         key-fixer
+                         (not (eq key-equiv 'equal))
+                         `((defcong ,key-equiv equal (,updater ,key ,val ,hash-table) 1
+                             :hints
+                             (("Goal"
+                               :by (:functional-instance
+                                    ,(if copyable
+                                         'lem-hash-table$a::key-equiv-implies-equal-updater/copyable-1
+                                         'lem-hash-table$a::key-equiv-implies-equal-updater/unique-1)
+                                    ,@fi-bindings))))))
+
+                  ,@(and val-recognizer
+                         val-fixer
+                         (not (eq val-equiv 'equal))
+                         `((defcong ,val-equiv equal (,updater ,key ,val ,hash-table) 2
+                             :hints
+                             (("Goal"
+                               :by (:functional-instance
+                                    ,(if copyable
+                                         'lem-hash-table$a::val-equiv-implies-equal-updater/copyable-2
+                                         'lem-hash-table$a::val-equiv-implies-equal-updater/unique-2)
+                                    ,@fi-bindings))))))
+
+                  (defcong ,equiv equal (,updater ,key ,val ,hash-table) 3
+                    :hints
+                    (("Goal"
+                      :by (:functional-instance
+                           ,(if copyable
+                                'lem-hash-table$a::equiv/copyable-implies-equal-updater/copyable-3
+                                'lem-hash-table$a::equiv/unique-implies-equal-updater/unique-3)
                            ,@fi-bindings))))
 
                   ,@(and key-recognizer
@@ -1354,58 +2365,11 @@
                                 'lem-hash-table$a::updater/unique-when-not-recognizer/unique)
                            ,@fi-bindings))))
 
-                  ,@(and key-fixer
-                         `((defthm ,updater-of-key-fixer
-                             (equal (,updater (,key-fixer ,key) ,val ,hash-table)
-                                    (,updater ,key ,val ,hash-table))
-                             :hints
-                             (("Goal"
-                               :by (:functional-instance
-                                    ,(if copyable
-                                         'lem-hash-table$a::updater/copyable-of-key-fixer
-                                         'lem-hash-table$a::updater/unique-of-key-fixer)
-                                    ,@fi-bindings))))))
-
-                  ,@(and val-fixer
-                         `((defthm ,updater-of-val-fixer
-                             (equal (,updater ,key (,val-fixer ,val) ,hash-table)
-                                    (,updater ,key ,val ,hash-table))
-                             :hints
-                             (("Goal"
-                               :by (:functional-instance
-                                    ,(if copyable
-                                         'lem-hash-table$a::updater/copyable-of-val-fixer
-                                         'lem-hash-table$a::updater/unique-of-val-fixer)
-                                    ,@fi-bindings))))))
-
-                  (defthm ,updater-of-fixer
-                    (equal (,updater ,key ,val (,fixer ,hash-table))
-                           (,updater ,key ,val ,hash-table))
-                    :hints
-                    (("Goal"
-                      :by (:functional-instance
-                           ,(if copyable
-                                'lem-hash-table$a::updater/copyable-of-fixer/copyable
-                                'lem-hash-table$a::updater/unique-of-fixer/unique)
-                           ,@fi-bindings))))
-
                   (defthmd ,updater-of-accessor-when-boundp-free
                     (implies (and (,boundp ,key ,hash-table)
-                                  (equal ,(if val-fixer
-                                              `(,val-fixer ,val)
-                                              val)
-                                         (,accessor ,key ,hash-table)))
+                                  (,val-equiv ,val (,accessor ,key ,hash-table)))
                              (equal (,updater ,key ,val ,hash-table)
                                     (,fixer ,hash-table)))
-                    :rule-classes
-                    ((:rewrite :corollary
-                               (implies (and (,boundp ,key ,hash-table)
-                                             (case-split (equal ,(if val-fixer
-                                                                     `(,val-fixer ,val)
-                                                                     val)
-                                                                (,accessor ,key ,hash-table))))
-                                        (equal (,updater ,key ,val ,hash-table)
-                                               (,fixer ,hash-table)))))
                     :hints
                     (("Goal"
                       :by (:functional-instance
@@ -1415,24 +2379,14 @@
                            ,@fi-bindings))))
 
                   (defthmd ,updater-of-accessor
-                    (implies (equal ,(if key-fixer
-                                         `(,key-fixer ,%key)
-                                         %key)
-                                    ,(if key-fixer
-                                         `(,key-fixer ,key)
-                                         key))
+                    (implies (,key-equiv ,%key ,key)
                              (equal (,updater ,%key (,accessor ,key ,hash-table) ,hash-table)
                                     (if (,boundp ,%key ,hash-table)
                                         (,fixer ,hash-table)
                                         (,updater ,%key ,default-val ,hash-table))))
                     :rule-classes
                     ((:rewrite :corollary
-                               (implies (case-split (equal ,(if key-fixer
-                                                                `(,key-fixer ,%key)
-                                                                %key)
-                                                           ,(if key-fixer
-                                                                `(,key-fixer ,key)
-                                                                key)))
+                               (implies (case-split (,key-equiv ,%key ,key))
                                         (equal (,updater ,%key (,accessor ,key ,hash-table) ,hash-table)
                                                (if (,boundp ,%key ,hash-table)
                                                    (,fixer ,hash-table)
@@ -1447,13 +2401,9 @@
 
                   (defthm ,updater-of-accessor-when-boundp
                     (implies (and (,boundp ,%key ,hash-table)
-                                  (equal ,(if key-fixer
-                                              `(,key-fixer ,%key)
-                                              %key)
-                                         ,(if key-fixer
-                                              `(,key-fixer ,key)
-                                              key)))
-                             (equal (,updater ,%key (,accessor ,key ,hash-table) ,hash-table)
+                                  (,key-equiv ,%key ,key)
+                                  (,equiv ,%hash-table ,hash-table))
+                             (equal (,updater ,%key (,accessor ,key ,%hash-table) ,hash-table)
                                     (,fixer ,hash-table)))
                     :hints
                     (("Goal"
@@ -1465,12 +2415,7 @@
 
                   (defthm ,updater-of-accessor-when-not-boundp
                     (implies (and (not (,boundp ,%key ,hash-table))
-                                  (equal ,(if key-fixer
-                                              `(,key-fixer ,%key)
-                                              %key)
-                                         ,(if key-fixer
-                                              `(,key-fixer ,key)
-                                              key)))
+                                  (,key-equiv ,%key ,key))
                              (equal (,updater ,%key (,accessor ,key ,hash-table) ,hash-table)
                                     (,updater ,%key ,default-val ,hash-table)))
                     :hints
@@ -1483,12 +2428,7 @@
 
                   (defthmd ,updater-of-updater
                     (equal (,updater ,%key ,%val (,updater ,key ,val ,hash-table))
-                           (if (equal ,(if key-fixer
-                                           `(,key-fixer ,%key)
-                                           %key)
-                                      ,(if key-fixer
-                                           `(,key-fixer ,key)
-                                           key))
+                           (if (,key-equiv ,%key ,key)
                                (,updater ,%key ,%val ,hash-table)
                                (,updater ,key ,val (,updater ,%key ,%val ,hash-table))))
                     :rule-classes
@@ -1502,12 +2442,7 @@
                            ,@fi-bindings))))
 
                   (defthm ,updater-of-updater-same
-                    (implies (equal ,(if key-fixer
-                                         `(,key-fixer ,%key)
-                                         %key)
-                                    ,(if key-fixer
-                                         `(,key-fixer ,key)
-                                         key))
+                    (implies (,key-equiv ,%key ,key)
                              (equal (,updater ,%key ,%val (,updater ,key ,val ,hash-table))
                                     (,updater ,%key ,%val ,hash-table)))
                     :hints
@@ -1519,12 +2454,7 @@
                            ,@fi-bindings))))
 
                   (defthm ,updater-of-updater-diff
-                    (implies (not (equal ,(if key-fixer
-                                              `(,key-fixer ,%key)
-                                              %key)
-                                         ,(if key-fixer
-                                              `(,key-fixer ,key)
-                                              key)))
+                    (implies (not (,key-equiv ,%key ,key))
                              (equal (,updater ,%key ,%val (,updater ,key ,val ,hash-table))
                                     (,updater ,key ,val (,updater ,%key ,%val ,hash-table))))
                     :rule-classes
@@ -1538,14 +2468,16 @@
                            ,@fi-bindings))))
 
                   (defthm ,updater-of-remover-same
-                    (implies (equal ,(if key-fixer
-                                         `(,key-fixer ,%key)
-                                         %key)
-                                    ,(if key-fixer
-                                         `(,key-fixer ,key)
-                                         key))
+                    (implies (,key-equiv ,%key ,key)
                              (equal (,updater ,%key ,val (,remover ,key ,hash-table))
                                     (,updater ,%key ,val ,hash-table)))
+                    :rule-classes
+                    ((:rewrite :corollary
+                               (implies (,key-equiv ,%key ,(if (eq key-equiv 'equal)
+                                                               key
+                                                               `(double-rewrite ,key)))
+                                        (equal (,updater ,%key ,val (,remover ,key ,hash-table))
+                                               (,updater ,%key ,val (double-rewrite ,hash-table))))))
                     :hints
                     (("Goal"
                       :by (:functional-instance
@@ -1564,6 +2496,27 @@
                            ,(if copyable
                                 'lem-hash-table$a::boundp/copyable-tp
                                 'lem-hash-table$a::boundp/unique-tp)
+                           ,@fi-bindings))))
+
+                  ,@(and key-recognizer
+                         key-fixer
+                         (not (eq key-equiv 'equal))
+                         `((defcong ,key-equiv equal (,boundp ,key ,hash-table) 1
+                             :hints
+                             (("Goal"
+                               :by (:functional-instance
+                                    ,(if copyable
+                                         'lem-hash-table$a::key-equiv-implies-equal-boundp/copyable-1
+                                         'lem-hash-table$a::key-equiv-implies-equal-boundp/unique-1)
+                                    ,@fi-bindings))))))
+
+                  (defcong ,equiv equal (,boundp ,key ,hash-table) 2
+                    :hints
+                    (("Goal"
+                      :by (:functional-instance
+                           ,(if copyable
+                                'lem-hash-table$a::equiv/copyable-implies-equal-boundp/copyable-2
+                                'lem-hash-table$a::equiv/unique-implies-equal-boundp/unique-2)
                            ,@fi-bindings))))
 
                   ,@(and key-recognizer
@@ -1600,37 +2553,9 @@
                                 'lem-hash-table$a::boundp/unique-of-creator/unique)
                            ,@fi-bindings))))
 
-                  ,@(and key-fixer
-                         `((defthm ,boundp-of-key-fixer
-                             (equal (,boundp (,key-fixer ,key) ,hash-table)
-                                    (,boundp ,key ,hash-table))
-                             :hints
-                             (("Goal"
-                               :by (:functional-instance
-                                    ,(if copyable
-                                         'lem-hash-table$a::boundp/copyable-of-key-fixer
-                                         'lem-hash-table$a::boundp/unique-of-key-fixer)
-                                    ,@fi-bindings))))))
-
-                  (defthm ,boundp-of-fixer
-                    (equal (,boundp ,key (,fixer ,hash-table))
-                           (,boundp ,key ,hash-table))
-                    :hints
-                    (("Goal"
-                      :by (:functional-instance
-                           ,(if copyable
-                                'lem-hash-table$a::boundp/copyable-of-fixer/copyable
-                                'lem-hash-table$a::boundp/unique-of-fixer/unique)
-                           ,@fi-bindings))))
-
                   (defthmd ,boundp-of-updater
                     (equal (,boundp ,%key (,updater ,key ,val ,hash-table))
-                           (if (equal ,(if key-fixer
-                                           `(,key-fixer ,%key)
-                                           %key)
-                                      ,(if key-fixer
-                                           `(,key-fixer ,key)
-                                           key))
+                           (if (,key-equiv ,%key ,key)
                                t
                                (,boundp ,%key ,hash-table)))
                     :hints
@@ -1642,12 +2567,7 @@
                            ,@fi-bindings))))
 
                   (defthm ,boundp-of-updater-same
-                    (implies (equal ,(if key-fixer
-                                         `(,key-fixer ,%key)
-                                         %key)
-                                    ,(if key-fixer
-                                         `(,key-fixer ,key)
-                                         key))
+                    (implies (,key-equiv ,%key ,key)
                              (equal (,boundp ,%key (,updater ,key ,val ,hash-table))
                                     t))
                     :hints
@@ -1659,12 +2579,7 @@
                            ,@fi-bindings))))
 
                   (defthm ,boundp-of-updater-diff
-                    (implies (not (equal ,(if key-fixer
-                                              `(,key-fixer ,%key)
-                                              %key)
-                                         ,(if key-fixer
-                                              `(,key-fixer ,key)
-                                              key)))
+                    (implies (not (,key-equiv ,%key ,key))
                              (equal (,boundp ,%key (,updater ,key ,val ,hash-table))
                                     (,boundp ,%key ,hash-table)))
                     :hints
@@ -1677,14 +2592,17 @@
 
                   (defthmd ,boundp-of-remover
                     (equal (,boundp ,%key (,remover ,key ,hash-table))
-                           (if (equal ,(if key-fixer
-                                           `(,key-fixer ,%key)
-                                           %key)
-                                      ,(if key-fixer
-                                           `(,key-fixer ,key)
-                                           key))
+                           (if (,key-equiv ,%key ,key)
                                nil
                                (,boundp ,%key ,hash-table)))
+                    :rule-classes
+                    ((:rewrite :corollary
+                               (equal (,boundp ,%key (,remover ,key ,hash-table))
+                                      (if (,key-equiv ,%key ,(if (eq key-equiv 'equal)
+                                                                 key
+                                                                 `(double-rewrite ,key)))
+                                          nil
+                                          (,boundp ,%key (double-rewrite ,hash-table))))))
                     :hints
                     (("Goal"
                       :by (:functional-instance
@@ -1694,13 +2612,14 @@
                            ,@fi-bindings))))
 
                   (defthm ,boundp-of-remover-same
-                    (implies (equal ,(if key-fixer
-                                         `(,key-fixer ,%key)
-                                         %key)
-                                    ,(if key-fixer
-                                         `(,key-fixer ,key)
-                                         key))
+                    (implies (,key-equiv ,%key ,key)
                              (not (,boundp ,%key (,remover ,key ,hash-table))))
+                    :rule-classes
+                    ((:rewrite :corollary
+                               (implies (,key-equiv ,%key ,(if (eq key-equiv 'equal)
+                                                               key
+                                                               `(double-rewrite ,key)))
+                                        (not (,boundp ,%key (,remover ,key ,hash-table))))))
                     :hints
                     (("Goal"
                       :by (:functional-instance
@@ -1710,14 +2629,16 @@
                            ,@fi-bindings))))
 
                   (defthm ,boundp-of-remover-diff
-                    (implies (not (equal ,(if key-fixer
-                                              `(,key-fixer ,%key)
-                                              %key)
-                                         ,(if key-fixer
-                                              `(,key-fixer ,key)
-                                              key)))
+                    (implies (not (,key-equiv ,%key ,key))
                              (equal (,boundp ,%key (,remover ,key ,hash-table))
                                     (,boundp ,%key ,hash-table)))
+                    :rule-classes
+                    ((:rewrite :corollary
+                               (implies (not (,key-equiv ,%key ,(if (eq key-equiv 'equal)
+                                                                    key
+                                                                    `(double-rewrite ,key))))
+                                        (equal (,boundp ,%key (,remover ,key ,hash-table))
+                                               (,boundp ,%key (double-rewrite ,hash-table))))))
                     :hints
                     (("Goal"
                       :by (:functional-instance
@@ -1726,26 +2647,30 @@
                                 'lem-hash-table$a::boundp/unique-of-remover/unique-diff)
                            ,@fi-bindings))))
 
-                  (defthmd ,boundp-when-zp-count
-                    (implies (zp (,count ,hash-table))
-                             (not (,boundp ,key ,hash-table)))
-                    :hints
-                    (("Goal"
-                      :by (:functional-instance
-                           ,(if copyable
-                                'lem-hash-table$a::boundp/copyable-when-zp-count/copyable
-                                'lem-hash-table$a::boundp/unique-when-zp-count/unique)
-                           ,@fi-bindings))))
-
                   ,@(and copyable
                          `((defthm ,boundp-of-keys-set
                              (equal (,boundp ,key (,keys-set ,set ,hash-table))
                                     (,boundp ,key ,hash-table))
+                             :rule-classes
+                             ((:rewrite :corollary
+                                        (equal (,boundp ,key (,keys-set ,set ,hash-table))
+                                               (,boundp ,key (double-rewrite ,hash-table)))))
                              :hints
                              (("Goal"
                                :by (:functional-instance
                                     lem-hash-table$a::boundp/copyable-of-keys-set
                                     ,@fi-bindings))))))
+
+                  (defthmd ,boundp-when-count-is-zero
+                    (implies (equal (,count ,hash-table) 0)
+                             (not (,boundp ,key ,hash-table)))
+                    :hints
+                    (("Goal"
+                      :by (:functional-instance
+                           ,(if copyable
+                                'lem-hash-table$a::boundp/copyable-when-count/copyable-is-zero
+                                'lem-hash-table$a::boundp/unique-when-count/unique-is-zero)
+                           ,@fi-bindings))))
 
                   ;; `GETP'
                   (defthm ,getp-tp
@@ -1765,6 +2690,12 @@
                             (,getp ,key ,hash-table)
                       (and (equal v0 (,accessor ,key ,hash-table))
                            (equal v1 (,boundp ,key ,hash-table))))
+                    :rule-classes
+                    ((:rewrite :corollary
+                               (mv-let (v0 v1)
+                                       (,getp ,key ,hash-table)
+                                 (and (equal v0 (,accessor (double-rewrite ,key) (double-rewrite ,hash-table)))
+                                      (equal v1 (,boundp (double-rewrite ,key) (double-rewrite ,hash-table)))))))
                     :hints
                     (("Goal"
                       :by (:functional-instance
@@ -1786,6 +2717,27 @@
                            ,(if copyable
                                 'lem-hash-table$a::remover/copyable-tp
                                 'lem-hash-table$a::remover/unique-tp)
+                           ,@fi-bindings))))
+
+                  ,@(and key-recognizer
+                         key-fixer
+                         (not (eq key-equiv 'equal))
+                         `((defcong ,key-equiv equal (,remover ,key ,hash-table) 1
+                             :hints
+                             (("Goal"
+                               :by (:functional-instance
+                                    ,(if copyable
+                                         'lem-hash-table$a::key-equiv-implies-equal-remover/copyable-1
+                                         'lem-hash-table$a::key-equiv-implies-equal-remover/unique-1)
+                                    ,@fi-bindings))))))
+
+                  (defcong ,equiv equal (,remover ,key ,hash-table) 2
+                    :hints
+                    (("Goal"
+                      :by (:functional-instance
+                           ,(if copyable
+                                'lem-hash-table$a::equiv/copyable-implies-equal-remover/copyable-2
+                                'lem-hash-table$a::equiv/unique-implies-equal-remover/unique-2)
                            ,@fi-bindings))))
 
                   ,@(and key-recognizer
@@ -1824,37 +2776,9 @@
                                 'lem-hash-table$a::remover/unique-of-creator/unique)
                            ,@fi-bindings))))
 
-                  ,@(and key-fixer
-                         `((defthm ,remover-of-key-fixer
-                             (equal (,remover (,key-fixer ,key) ,hash-table)
-                                    (,remover ,key ,hash-table))
-                             :hints
-                             (("Goal"
-                               :by (:functional-instance
-                                    ,(if copyable
-                                         'lem-hash-table$a::remover/copyable-of-key-fixer
-                                         'lem-hash-table$a::remover/unique-of-key-fixer)
-                                    ,@fi-bindings))))))
-
-                  (defthm ,remover-of-fixer
-                    (equal (,remover ,key (,fixer ,hash-table))
-                           (,remover ,key ,hash-table))
-                    :hints
-                    (("Goal"
-                      :by (:functional-instance
-                           ,(if copyable
-                                'lem-hash-table$a::remover/copyable-of-fixer/copyable
-                                'lem-hash-table$a::remover/unique-of-fixer/unique)
-                           ,@fi-bindings))))
-
                   (defthmd ,remover-of-updater
                     (equal (,remover ,%key (,updater ,key ,val ,hash-table))
-                           (if (equal ,(if key-fixer
-                                           `(,key-fixer ,%key)
-                                           %key)
-                                      ,(if key-fixer
-                                           `(,key-fixer ,key)
-                                           key))
+                           (if (,key-equiv ,%key ,key)
                                (,remover ,%key ,hash-table)
                                (,updater ,key ,val (,remover ,%key ,hash-table))))
                     :hints
@@ -1866,12 +2790,7 @@
                            ,@fi-bindings))))
 
                   (defthm ,remover-of-updater-same
-                    (implies (equal ,(if key-fixer
-                                         `(,key-fixer ,%key)
-                                         %key)
-                                    ,(if key-fixer
-                                         `(,key-fixer ,key)
-                                         key))
+                    (implies (,key-equiv ,%key ,key)
                              (equal (,remover ,%key (,updater ,key ,val ,hash-table))
                                     (,remover ,%key ,hash-table)))
                     :hints
@@ -1883,12 +2802,7 @@
                            ,@fi-bindings))))
 
                   (defthm ,remover-of-updater-diff
-                    (implies (not (equal ,(if key-fixer
-                                              `(,key-fixer ,%key)
-                                              %key)
-                                         ,(if key-fixer
-                                              `(,key-fixer ,key)
-                                              key)))
+                    (implies (not (,key-equiv ,%key ,key))
                              (equal (,remover ,%key (,updater ,key ,val ,hash-table))
                                     (,updater ,key ,val (,remover ,%key ,hash-table))))
                     :hints
@@ -1913,12 +2827,7 @@
 
                   (defthmd ,remover-of-remover
                     (equal (,remover ,%key (,remover ,key ,hash-table))
-                           (if (equal ,(if key-fixer
-                                           `(,key-fixer ,%key)
-                                           %key)
-                                      ,(if key-fixer
-                                           `(,key-fixer ,key)
-                                           key))
+                           (if (,key-equiv ,%key ,key)
                                (,remover ,%key ,hash-table)
                                (,remover ,key (,remover ,%key ,hash-table))))
                     :rule-classes
@@ -1932,12 +2841,7 @@
                            ,@fi-bindings))))
 
                   (defthm ,remover-of-remover-same
-                    (implies (equal ,(if key-fixer
-                                         `(,key-fixer ,%key)
-                                         %key)
-                                    ,(if key-fixer
-                                         `(,key-fixer ,key)
-                                         key))
+                    (implies (,key-equiv ,%key ,key)
                              (equal (,remover ,%key (,remover ,key ,hash-table))
                                     (,remover ,%key ,hash-table)))
                     :hints
@@ -1949,12 +2853,7 @@
                            ,@fi-bindings))))
 
                   (defthm ,remover-of-remover-diff
-                    (implies (not (equal ,(if key-fixer
-                                              `(,key-fixer ,%key)
-                                              %key)
-                                         ,(if key-fixer
-                                              `(,key-fixer ,key)
-                                              key)))
+                    (implies (not (,key-equiv ,%key ,key))
                              (equal (,remover ,%key (,remover ,key ,hash-table))
                                     (,remover ,key (,remover ,%key ,hash-table))))
                     :rule-classes
@@ -1967,6 +2866,21 @@
                                 'lem-hash-table$a::remover/unique-of-remover/unique-diff)
                            ,@fi-bindings))))
 
+                  (defthmd ,remover-when-count-is-zero
+                    (implies (equal (,count ,hash-table) 0)
+                             (equal (,remover ,key ,hash-table)
+                                    ,(if copyable
+                                         `(,keys-set (,keys ,hash-table)
+                                                     (,creator))
+                                         `(,creator))))
+                    :hints
+                    (("Goal"
+                      :by (:functional-instance
+                           ,(if copyable
+                                'lem-hash-table$a::remover/copyable-when-count/copyable-is-zero
+                                'lem-hash-table$a::remover/unique-when-count/unique-is-zero)
+                           ,@fi-bindings))))
+
                   ;; `COUNT'
                   (defthm ,count-tp
                     (natp (,count ,hash-table))
@@ -1977,6 +2891,15 @@
                            ,(if copyable
                                 'lem-hash-table$a::count/copyable-tp
                                 'lem-hash-table$a::count/unique-tp)
+                           ,@fi-bindings))))
+
+                  (defcong ,equiv equal (,count ,hash-table) 1
+                    :hints
+                    (("Goal"
+                      :by (:functional-instance
+                           ,(if copyable
+                                'lem-hash-table$a::equiv/copyable-implies-equal-count/copyable-1
+                                'lem-hash-table$a::equiv/unique-implies-equal-count/unique-1)
                            ,@fi-bindings))))
 
                   (defthmd ,count-when-not-recognizer
@@ -2000,17 +2923,6 @@
                            ,(if copyable
                                 'lem-hash-table$a::count/copyable-of-creator/copyable
                                 'lem-hash-table$a::count/unique-of-creator/unique)
-                           ,@fi-bindings))))
-
-                  (defthm ,count-of-fixer
-                    (equal (,count (,fixer ,hash-table))
-                           (,count ,hash-table))
-                    :hints
-                    (("Goal"
-                      :by (:functional-instance
-                           ,(if copyable
-                                'lem-hash-table$a::count/copyable-of-fixer/copyable
-                                'lem-hash-table$a::count/unique-of-fixer/unique)
                            ,@fi-bindings))))
 
                   (defthmd ,count-of-updater
@@ -2050,7 +2962,7 @@
                                 'lem-hash-table$a::count/unique-of-updater/unique-when-not-boundp/unique)
                            ,@fi-bindings))))
 
-                  (defthm ,count-when-boundp
+                  (defthmd ,count-when-boundp
                     (implies (,boundp ,key ,hash-table)
                              (posp (,count ,hash-table)))
                     :rule-classes :type-prescription
@@ -2103,11 +3015,41 @@
                          `((defthm ,count-of-keys-set
                              (equal (,count (,keys-set ,set ,hash-table))
                                     (,count ,hash-table))
+                             :rule-classes
+                             ((:rewrite :corollary
+                                        (equal (,count (,keys-set ,set ,hash-table))
+                                               (,count (double-rewrite ,hash-table)))))
                              :hints
                              (("Goal"
                                :by (:functional-instance
                                     lem-hash-table$a::count/copyable-of-keys-set
                                     ,@fi-bindings))))))
+
+                  (defthm ,creator-when-count-is-zero
+                    (implies ,(if copyable
+                                  `(and (set::emptyp (,keys ,hash-table))
+                                        (equal (,count ,hash-table) 0))
+                                  `(equal (,count ,hash-table) 0))
+                             (,equiv ,hash-table (,creator)))
+                    :rule-classes
+                    ((:forward-chaining :trigger-terms
+                                        ((,count ,hash-table)
+                                         ,@(and copyable
+                                                `((set::emptyp (,keys ,hash-table)))))
+                                        :corollary
+                                        (implies t
+                                                 (implies ,(if copyable
+                                                               `(and (set::emptyp (,keys ,hash-table))
+                                                                     (equal (,count ,hash-table) 0))
+                                                               `(equal (,count ,hash-table) 0))
+                                                          (,equiv ,hash-table (,creator))))))
+                    :hints
+                    (("Goal"
+                      :by (:functional-instance
+                           ,(if copyable
+                                'lem-hash-table$a::creator/copyable-when-count/copyable-is-zero
+                                'lem-hash-table$a::creator/unique-when-count/unique-is-zero)
+                           ,@fi-bindings))))
 
                   ;; `CLEAR'
                   (defthm ,clear-tp
@@ -2161,177 +3103,6 @@
                                 'lem-hash-table$a::init/unique-rw)
                            ,@fi-bindings))))
 
-                  ;; `KEYSP'
-                  ,@(and copyable
-                         key-recognizer
-                         `((defthm ,keysp-tp
-                             (booleanp (,keysp ,set))
-                             :rule-classes :type-prescription
-                             :hints
-                             (("Goal"
-                               :by (:functional-instance
-                                    lem-hash-table$a::keysp-tp
-                                    ,@fi-bindings))))
-
-                           (defthm ,keysp-cr
-                             (implies (,keysp ,set)
-                                      (true-listp ,set))
-                             :rule-classes :compound-recognizer
-                             :hints
-                             (("Goal"
-                               :by (:functional-instance
-                                    lem-hash-table$a::keysp-cr
-                                    ,@fi-bindings))))
-
-                           (defthmd ,keysp-def
-                             (equal (,keysp ,set)
-                                    (and (set::setp ,set)
-                                         (or (set::emptyp ,set)
-                                             (and (,key-recognizer (set::head ,set))
-                                                  (,keysp (set::tail ,set))))))
-                             :rule-classes
-                             ((:definition :controller-alist ((,keysp t))))
-                             :hints
-                             (("Goal"
-                               :by (:functional-instance
-                                    lem-hash-table$a::keysp-def
-                                    ,@fi-bindings))))
-
-                           (defthm ,keysp-when-emptyp
-                             (implies (set::emptyp ,set)
-                                      (equal (,keysp ,set)
-                                             (set::setp ,set)))
-                             :hints
-                             (("Goal"
-                               :by (:functional-instance
-                                    lem-hash-table$a::keysp-when-emptyp
-                                    ,@fi-bindings))))
-
-                           (defthm ,keysp-of-keys-fix
-                             (,keysp (,keys-fix ,set))
-                             :hints
-                             (("Goal"
-                               :by (:functional-instance
-                                    lem-hash-table$a::keysp-of-keys-fix
-                                    ,@fi-bindings))))
-
-                           (defthm ,setp-when-keysp
-                             (implies (,keysp ,set)
-                                      (set::setp ,set))
-                             :hints
-                             (("Goal"
-                               :by (:functional-instance
-                                    lem-hash-table$a::setp-when-keysp
-                                    ,@fi-bindings))))
-
-                           (defthm ,key-recognizer-of-head-when-keysp
-                             (implies (and (,keysp ,set)
-                                           (not (set::emptyp ,set)))
-                                      (,key-recognizer (set::head ,set)))
-                             :hints
-                             (("Goal"
-                               :by (:functional-instance
-                                    lem-hash-table$a::key-recognizer-of-head-when-keysp
-                                    ,@fi-bindings))))
-
-                           (defthm ,keysp-of-tail-when-keysp
-                             (implies (and (,keysp ,set)
-                                           (not (set::emptyp ,set)))
-                                      (,keysp (set::tail ,set)))
-                             :hints
-                             (("Goal"
-                               :by (:functional-instance
-                                    lem-hash-table$a::keysp-of-tail-when-keysp
-                                    ,@fi-bindings))))
-
-                           (defthmd ,in-when-keysp-split
-                             (implies (and (,keysp ,set)
-                                           (not (,key-recognizer ,key)))
-                                      (not (set::in ,key ,set)))
-                             :rule-classes
-                             ((:rewrite :corollary
-                                        (implies (and (,keysp ,set)
-                                                      (not (case-split (,key-recognizer ,key))))
-                                                 (not (set::in ,key ,set)))))
-                             :hints
-                             (("Goal"
-                               :by (:functional-instance
-                                    lem-hash-table$a::in-when-keysp
-                                    ,@fi-bindings))))
-
-                           (defthm ,in-when-keysp
-                             (implies (and (,keysp ,set)
-                                           (not (,key-recognizer ,key)))
-                                      (not (set::in ,key ,set)))
-                             :hints
-                             (("Goal"
-                               :by (:functional-instance
-                                    lem-hash-table$a::in-when-keysp
-                                    ,@fi-bindings))))
-
-                           (defthm ,keysp-when-subset
-                             (implies (and (not (,keysp ,%set))
-                                           (,keysp ,set))
-                                      (equal (set::subset ,%set ,set)
-                                             (set::emptyp ,%set)))
-                             :hints
-                             (("Goal"
-                               :by (:functional-instance
-                                    lem-hash-table$a::keysp-when-subset
-                                    ,@fi-bindings))))
-
-
-                           (defthm ,keysp-of-insert
-                             (equal (,keysp (set::insert key set))
-                                    (and (,key-recognizer key)
-                                         (or (set::emptyp set)
-                                             (,keysp set))))
-                             :hints
-                             (("Goal"
-                               :by (:functional-instance
-                                    lem-hash-table$a::keysp-of-insert
-                                    ,@fi-bindings))))
-
-                           (defthm ,keysp-of-delete
-                             (implies (,keysp ,set)
-                                      (,keysp (set::delete ,key ,set)))
-                             :hints
-                             (("Goal"
-                               :by (:functional-instance
-                                    lem-hash-table$a::keysp-of-delete
-                                    ,@fi-bindings))))))
-
-                  ;; `KEYS-FIX'
-                  ,@(and copyable
-                         key-recognizer
-                         `((defthm ,keys-fix-tp
-                             (true-listp (,keys-fix ,set))
-                             :rule-classes :type-prescription
-                             :hints
-                             (("Goal"
-                               :by (:functional-instance
-                                    lem-hash-table$a::keys-fix-tp
-                                    ,@fi-bindings))))
-
-                           (defthm ,keys-fix-when-keysp
-                             (implies (,keysp ,set)
-                                      (equal (,keys-fix ,set)
-                                             ,set))
-                             :hints
-                             (("Goal"
-                               :by (:functional-instance
-                                    lem-hash-table$a::keys-fix-when-keysp
-                                    ,@fi-bindings))))
-
-                           (defthm ,keys-fix-when-not-keysp
-                             (implies (not (,keysp ,set))
-                                      (not (,keys-fix ,set)))
-                             :hints
-                             (("Goal"
-                               :by (:functional-instance
-                                    lem-hash-table$a::keys-fix-when-not-keysp
-                                    ,@fi-bindings))))))
-
                   ;; `KEYS'
                   ,@(and copyable
                          `((defthm ,keys-tp
@@ -2343,14 +3114,11 @@
                                     lem-hash-table$a::keys-tp
                                     ,@fi-bindings))))
 
-                           (defthm ,keysp-of-keys
-                             ,(if key-recognizer
-                                  `(,keysp (,keys ,hash-table))
-                                  `(set::setp (,keys ,hash-table)))
+                           (defcong ,equiv equal (,keys ,hash-table) 1
                              :hints
                              (("Goal"
                                :by (:functional-instance
-                                    lem-hash-table$a::keysp-of-keys
+                                    lem-hash-table$a::equiv/copyable-implies-equal-keys-1
                                     ,@fi-bindings))))
 
                            (defthmd ,keys-when-not-recognizer
@@ -2368,15 +3136,6 @@
                              (("Goal"
                                :by (:functional-instance
                                     lem-hash-table$a::keys-of-creator/copyable
-                                    ,@fi-bindings))))
-
-                           (defthm ,keys-of-fixer
-                             (equal (,keys (,fixer ,hash-table))
-                                    (,keys ,hash-table))
-                             :hints
-                             (("Goal"
-                               :by (:functional-instance
-                                    lem-hash-table$a::keys-of-fixer/copyable
                                     ,@fi-bindings))))
 
                            (defthm ,keys-of-updater
@@ -2399,9 +3158,13 @@
 
                            (defthm ,keys-of-keys-set
                              (equal (,keys (,keys-set ,set ,hash-table))
-                                    ,(if key-recognizer
-                                         `(,keys-fix ,set)
-                                         `(set::sfix ,set)))
+                                    (,keys-fix ,set))
+                             :rule-classes
+                             ((:rewrite :corollary
+                                        (equal (,keys (,keys-set ,set ,hash-table))
+                                               (,keys-fix ,(if (eq keysp 'set::setp)
+                                                               set
+                                                               `(double-rewrite ,set))))))
                              :hints
                              (("Goal"
                                :by (:functional-instance
@@ -2420,10 +3183,13 @@
                                     lem-hash-table$a::keys-set-tp
                                     ,@fi-bindings))))
 
+                           ,@(and (not (eq keys-equiv 'equal))
+                                  `((defcong ,keys-equiv equal (,keys-set ,set ,hash-table) 1)))
+
+                           (defcong ,equiv equal (,keys-set ,set ,hash-table) 2)
+
                            (defthmd ,keys-set-when-not-keysp
-                             (implies (not ,(if key-recognizer
-                                                `(,keysp ,set)
-                                                `(set::setp ,set)))
+                             (implies (not (,keysp ,set))
                                       (equal (,keys-set ,set ,hash-table)
                                              (,keys-set '() ,hash-table)))
                              :hints
@@ -2452,27 +3218,6 @@
                                     lem-hash-table$a::keys-set-of-creator/copyable
                                     ,@fi-bindings))))
 
-                           (defthm ,keys-set-of-keys-fix
-                             (equal (,keys-set ,(if key-recognizer
-                                                    `(,keys-fix ,set)
-                                                    `(set::sfix ,set))
-                                               ,hash-table)
-                                    (,keys-set ,set ,hash-table))
-                             :hints
-                             (("Goal"
-                               :by (:functional-instance
-                                    lem-hash-table$a::keys-set-of-keys-fix
-                                    ,@fi-bindings))))
-
-                           (defthm ,keys-set-of-fixer
-                             (equal (,keys-set ,set (,fixer ,hash-table))
-                                    (,keys-set ,set ,hash-table))
-                             :hints
-                             (("Goal"
-                               :by (:functional-instance
-                                    lem-hash-table$a::keys-set-of-fixer/copyable
-                                    ,@fi-bindings))))
-
                            (defthm ,keys-set-of-updater
                              (equal (,keys-set ,set (,updater ,key ,val ,hash-table))
                                     (,updater ,key ,val (,keys-set ,set ,hash-table)))
@@ -2492,20 +3237,9 @@
                                     ,@fi-bindings))))
 
                            (defthmd ,keys-set-of-keys-free
-                             (implies (equal ,(if key-recognizer
-                                                  `(,keys-fix ,set)
-                                                  `(set::sfix ,set))
-                                             (,keys ,hash-table))
+                             (implies (,keys-equiv ,set (,keys ,hash-table))
                                       (equal (,keys-set ,set ,hash-table)
                                              (,fixer ,hash-table)))
-                             :rule-classes
-                             ((:rewrite :corollary
-                                        (implies (case-split (equal ,(if key-recognizer
-                                                                         `(,keys-fix ,set)
-                                                                         `(set::sfix ,set))
-                                                                    (,keys ,hash-table)))
-                                                 (equal (,keys-set ,set ,hash-table)
-                                                        (,fixer ,hash-table)))))
                              :hints
                              (("Goal"
                                :by (:functional-instance
@@ -2513,8 +3247,9 @@
                                     ,@fi-bindings))))
 
                            (defthm ,keys-set-of-keys
-                             (equal (,keys-set (,keys ,hash-table) ,hash-table)
-                                    (,fixer ,hash-table))
+                             (implies (,equiv ,%hash-table ,hash-table)
+                                      (equal (,keys-set (,keys ,%hash-table) ,hash-table)
+                                             (,fixer ,hash-table)))
                              :hints
                              (("Goal"
                                :by (:functional-instance
@@ -2536,12 +3271,8 @@
                                                 (,recognizer ,hash-table))
                                     :verify-guards nil))
                     (forall ,key
-                      ,(if key-recognizer
-                           `(implies (,key-recognizer ,key)
-                                     (equal (,boundp ,key ,%hash-table)
-                                            (,boundp ,key ,hash-table)))
-                           `(equal (,boundp ,key ,%hash-table)
-                                   (,boundp ,key ,hash-table))))
+                      (equal (,boundp ,key ,%hash-table)
+                             (,boundp ,key ,hash-table)))
                     :rewrite :direct)
 
                   (defun-sk ,vals-equal (,%hash-table ,hash-table)
@@ -2549,12 +3280,8 @@
                                                 (,recognizer ,hash-table))
                                     :verify-guards nil))
                     (forall ,key
-                      ,(if key-recognizer
-                           `(implies (,key-recognizer ,key)
-                                     (equal (,accessor ,key ,%hash-table)
-                                            (,accessor ,key ,hash-table)))
-                           `(equal (,accessor ,key ,%hash-table)
-                                   (,accessor ,key ,hash-table))))
+                      (equal (,accessor ,key ,%hash-table)
+                             (,accessor ,key ,hash-table)))
                     :rewrite :direct)
 
                   (defun-nx ,hash-table-equal (,%hash-table ,hash-table)
@@ -2572,6 +3299,110 @@
 
                   (table equality ',hash-table ',hash-table-equal)
 
+                  (local
+                    (in-theory
+                      (disable ,hash-table-constraints)))
+
+                  (defthm ,hash-table-equal-constraints
+                    (and (equal (,keys-equal ,%hash-table ,hash-table)
+                                ((lambda (,key ,hash-table ,%hash-table)
+                                   (equal (,boundp ,key ,%hash-table)
+                                          (,boundp ,key ,hash-table)))
+                                 (,keys-equal-witness ,%hash-table ,hash-table)
+                                 ,hash-table ,%hash-table))
+                         (implies (,keys-equal ,%hash-table ,hash-table)
+                                  (equal (,boundp ,key ,%hash-table)
+                                         (,boundp ,key ,hash-table)))
+                         (equal (,vals-equal ,%hash-table ,hash-table)
+                                ((lambda (,key ,hash-table ,%hash-table)
+                                   (equal (,accessor ,key ,%hash-table)
+                                          (,accessor ,key ,hash-table)))
+                                 (,vals-equal-witness ,%hash-table ,hash-table)
+                                 ,hash-table ,%hash-table))
+                         (implies (,vals-equal ,%hash-table ,hash-table)
+                                  (equal (,accessor ,key ,%hash-table)
+                                         (,accessor ,key ,hash-table)))
+                         (equal (,hash-table-equal ,%hash-table ,hash-table)
+                                (if (,recognizer ,%hash-table)
+                                    (if (,recognizer ,hash-table)
+                                        ,(if copyable
+                                             `(if (equal (,keys ,%hash-table)
+                                                         (,keys ,hash-table))
+                                                  (if (equal (,count ,%hash-table)
+                                                             (,count ,hash-table))
+                                                      (if (,keys-equal ,%hash-table ,hash-table)
+                                                          (,vals-equal ,%hash-table ,hash-table)
+                                                          'nil)
+                                                      'nil)
+                                                  'nil)
+                                             `(if (equal (,count ,%hash-table)
+                                                         (,count ,hash-table))
+                                                  (if (,keys-equal ,%hash-table ,hash-table)
+                                                      (,vals-equal ,%hash-table ,hash-table)
+                                                      'nil)
+                                                  'nil))
+                                        'nil)
+                                    'nil)))
+                    :rule-classes
+                    ((:definition :corollary
+                         (equal (,keys-equal ,%hash-table ,hash-table)
+                                ((lambda (,key ,hash-table ,%hash-table)
+                                   (equal (,boundp ,key ,%hash-table)
+                                          (,boundp ,key ,hash-table)))
+                                 (,keys-equal-witness ,%hash-table ,hash-table)
+                                 ,hash-table ,%hash-table)))
+                     (:rewrite :corollary
+                               (implies (,keys-equal ,%hash-table ,hash-table)
+                                        (equal (,boundp ,key ,%hash-table)
+                                               (,boundp ,key ,hash-table))))
+                     (:definition :corollary
+                         (equal (,vals-equal ,%hash-table ,hash-table)
+                                ((lambda (,key ,hash-table ,%hash-table)
+                                   (equal (,accessor ,key ,%hash-table)
+                                          (,accessor ,key ,hash-table)))
+                                 (,vals-equal-witness ,%hash-table ,hash-table)
+                                 ,hash-table ,%hash-table)))
+                     (:rewrite :corollary
+                               (implies (,vals-equal ,%hash-table ,hash-table)
+                                        (equal (,accessor ,key ,%hash-table)
+                                               (,accessor ,key ,hash-table))))
+                     (:definition :corollary
+                         (equal (,hash-table-equal ,%hash-table ,hash-table)
+                                (if (,recognizer ,%hash-table)
+                                    (if (,recognizer ,hash-table)
+                                        ,(if copyable
+                                             `(if (equal (,keys ,%hash-table)
+                                                         (,keys ,hash-table))
+                                                  (if (equal (,count ,%hash-table)
+                                                             (,count ,hash-table))
+                                                      (if (,keys-equal ,%hash-table ,hash-table)
+                                                          (,vals-equal ,%hash-table ,hash-table)
+                                                          'nil)
+                                                      'nil)
+                                                  'nil)
+                                             `(if (equal (,count ,%hash-table)
+                                                         (,count ,hash-table))
+                                                  (if (,keys-equal ,%hash-table ,hash-table)
+                                                      (,vals-equal ,%hash-table ,hash-table)
+                                                      'nil)
+                                                  'nil))
+                                        'nil)
+                                    'nil))))
+                    :hints
+                    (("Goal"
+                      :in-theory (disable ,keys-equal-necc
+                                          ,vals-equal-necc)
+                      :use ((:instance ,keys-equal-necc)
+                            (:instance ,vals-equal-necc)))))
+
+                  (local
+                    (in-theory
+                      (disable ,keys-equal
+                               ,vals-equal
+                               ,hash-table-equal
+                               (:definition ,hash-table-equal-constraints . 1)
+                               (:definition ,hash-table-equal-constraints . 2))))
+
                   (defthm ,hash-table-equal-fc
                     (implies (,hash-table-equal ,%hash-table ,hash-table)
                              (equal ,%hash-table ,hash-table))
@@ -2584,58 +3415,31 @@
                                                           (equal ,%hash-table ,hash-table)))))
                     :hints
                     (("Goal"
-                      :in-theory (disable ,recognizer
-                                          ,creator
-                                          ,fixer
-                                          ,accessor
-                                          ,updater
-                                          ,boundp
-                                          ,getp
-                                          ,remover
-                                          ,count
-                                          ,clear
-                                          ,init
-                                          ,@(and copyable
-                                                 (list keys
-                                                       keys-set))
-                                          ,keys-equal
-                                          ,keys-equal-necc
-                                          ,vals-equal
-                                          ,vals-equal-necc)
                       :by (:functional-instance
                            ,(if copyable
                                 'lem-hash-table$a::equal/copyable-fc
                                 'lem-hash-table$a::equal/unique-fc)
                            ,@fi-bindings-with-skolem))
-                     ("Subgoal 4"
-                      :use ((:instance ,vals-equal-necc
-                                       (,%hash-table lem-hash-table$a::%hash-table)
-                                       (,hash-table lem-hash-table$a::hash-table)
-                                       (,key lem-hash-table$a::key))))
                      ("Subgoal 3"
-                      :expand (:free (,%hash-table ,hash-table)
-                                     (,vals-equal ,%hash-table ,hash-table)))
-                     ("Subgoal 2"
-                      :use ((:instance ,keys-equal-necc
-                                       (,%hash-table lem-hash-table$a::%hash-table)
-                                       (,hash-table lem-hash-table$a::hash-table)
-                                       (,key lem-hash-table$a::key))))
+                      :in-theory (enable (:definition ,hash-table-equal-constraints . 2)))
                      ("Subgoal 1"
-                      :expand (:free (,%hash-table ,hash-table)
-                                     (,keys-equal ,%hash-table ,hash-table)))))))
+                      :in-theory (enable (:definition ,hash-table-equal-constraints . 1)))))))
 
               (stobj$a-property `(,hash-table (,recognizer
                                                ,creator
-                                               ,fixer)
+                                               ,fixer
+                                               ,equiv)
                                               ((,key
                                                 ,key-recognizer
                                                 ,default-key-name
-                                                ,key-fixer)
+                                                ,key-fixer
+                                                ,key-equiv)
                                                (,val
                                                 ,val-recognizer
                                                 ,(and (not stobj-property)
                                                       default-val-name)
-                                                ,val-fixer)
+                                                ,val-fixer
+                                                ,val-equiv)
                                                (,test
                                                 ,copyable)
                                                (,accessor
@@ -2646,15 +3450,13 @@
                                                 ,count
                                                 ,clear
                                                 ,init
+                                                ;; HERE: update accesses to these
                                                 ,@(and copyable
-                                                       (list (if key-recognizer
-                                                                 keysp
-                                                                 'set::setp)
-                                                             (if key-recognizer
-                                                                 keys-fix
-                                                                 'set::sfix)
-                                                             keys
-                                                             keys-set)))))))
+                                                       `((,keys
+                                                          ,keys-set
+                                                          ,keysp
+                                                          ,keys-fix
+                                                          ,keys-equiv))))))))
 
          `(progn
             ,@prologue
