books/projects/atomic-stobjs/test/hash-table-a.lisp
@@ -30,6 +30,7 @@
 (in-package "ACL2")
 
 (include-book "std/basic/defs" :dir :system)
+(include-book "std/basic/arith-equiv-defs" :dir :system)
 (include-book "../constructors/hash-table-a")
 
 (defun null-symbol-fix (x)
@@ -45,6 +46,13 @@
   (implies (not (symbolp key))
            (not (null-symbol-fix key))))
 
+(defun null-symbol-equiv (x y)
+  (declare (xargs :guard t))
+  (equal (null-symbol-fix x)
+         (null-symbol-fix y)))
+
+(defequiv null-symbol-equiv)
+
 (defthm nfix-when-natp
   (implies (natp key)
            (equal (nfix key) key)))
@@ -52,6 +60,13 @@
 (defthm nfix-when-not-natp
   (implies (not (natp key))
            (equal (nfix key) 0)))
+
+(defun char-equiv (x y)
+  (declare (xargs :guard t))
+  (equal (char-fix x)
+         (char-fix y)))
+
+(defequiv char-equiv)
 
 (defun string-fix (x)
   (declare (xargs :guard t))
@@ -69,6 +84,13 @@
 (defthm string-fix-when-not-stringp
   (implies (not (stringp val))
            (equal (string-fix val) "")))
+
+(defun string-equiv (x y)
+  (declare (xargs :guard t))
+  (equal (string-fix x)
+         (string-fix y)))
+
+(defequiv string-equiv)
 
 (defun if-bool-fix (x)
   (declare (xargs :guard t))
@@ -89,33 +111,39 @@
 (atomic-stobjs::define-hash-table$a ht/0 eq
   :key-recognizer symbolp
   :key-fixer null-symbol-fix
+  :key-equiv null-symbol-equiv
   :default-key nil)
 
 (atomic-stobjs::define-hash-table$a ht/0-nil eq
   :key-recognizer symbolp
   :key-fixer null-symbol-fix
+  :key-equiv null-symbol-equiv
   :default-key nil
   :copyable nil)
 
 (atomic-stobjs::define-hash-table$a ht/1 eql
   :key-recognizer natp
   :key-fixer nfix
+  :key-equiv nat-equiv
   :default-key 0)
 
 (atomic-stobjs::define-hash-table$a ht/1-nil eql
   :key-recognizer natp
   :key-fixer nfix
+  :key-equiv nat-equiv
   :default-key 0
   :copyable nil)
 
 (atomic-stobjs::define-hash-table$a ht/2 eql
   :key-recognizer characterp
   :key-fixer char-fix
+  :key-equiv char-equiv
   :default-key #.acl2::*null-char*)
 
 (atomic-stobjs::define-hash-table$a ht/2-nil eql
   :key-recognizer characterp
   :key-fixer char-fix
+  :key-equiv char-equiv
   :default-key #.acl2::*null-char*
   :copyable nil)
 
@@ -134,73 +162,89 @@
 (atomic-stobjs::define-hash-table$a ht/0-string eq
   :key-recognizer symbolp
   :key-fixer null-symbol-fix
+  :key-equiv null-symbol-equiv
   :default-key nil
   :val-recognizer stringp
   :val-fixer string-fix
+  :val-equiv string-equiv
   :default-val "")
 
 (atomic-stobjs::define-hash-table$a ht/0-string-nil eq
   :key-recognizer symbolp
   :key-fixer null-symbol-fix
+  :key-equiv null-symbol-equiv
   :default-key nil
   :val-recognizer stringp
   :val-fixer string-fix
+  :val-equiv string-equiv
   :default-val ""
   :copyable nil)
 
 (atomic-stobjs::define-hash-table$a ht/1-string eql
   :key-recognizer natp
   :key-fixer nfix
+  :key-equiv nat-equiv
   :default-key 0
   :val-recognizer stringp
   :val-fixer string-fix
+  :val-equiv string-equiv
   :default-val "")
 
 (atomic-stobjs::define-hash-table$a ht/1-string-nil eql
   :key-recognizer natp
   :key-fixer nfix
+  :key-equiv nat-equiv
   :default-key 0
   :val-recognizer stringp
   :val-fixer string-fix
+  :val-equiv string-equiv
   :default-val ""
   :copyable nil)
 
 (atomic-stobjs::define-hash-table$a ht/2-string eql
   :key-recognizer characterp
   :key-fixer char-fix
+  :key-equiv char-equiv
   :default-key #.acl2::*null-char*
   :val-recognizer stringp
   :val-fixer string-fix
+  :val-equiv string-equiv
   :default-val "")
 
 (atomic-stobjs::define-hash-table$a ht/2-string-nil eql
   :key-recognizer characterp
   :key-fixer char-fix
+  :key-equiv char-equiv
   :default-key #.acl2::*null-char*
   :val-recognizer stringp
   :val-fixer string-fix
+  :val-equiv string-equiv
   :default-val ""
   :copyable nil)
 
 (atomic-stobjs::define-hash-table$a ht/3-string hons-equal
   :val-recognizer stringp
   :val-fixer string-fix
+  :val-equiv string-equiv
   :default-val "")
 
 (atomic-stobjs::define-hash-table$a ht/3-string-nil hons-equal
   :val-recognizer stringp
   :val-fixer string-fix
+  :val-equiv string-equiv
   :default-val ""
   :copyable nil)
 
 (atomic-stobjs::define-hash-table$a ht/4-string equal
   :val-recognizer stringp
   :val-fixer string-fix
+  :val-equiv string-equiv
   :default-val "")
 
 (atomic-stobjs::define-hash-table$a ht/4-string-nil equal
   :val-recognizer stringp
   :val-fixer string-fix
+  :val-equiv string-equiv
   :default-val ""
   :copyable nil)
 
@@ -209,73 +253,89 @@
 (atomic-stobjs::define-hash-table$a ht/0-boolean eq
   :key-recognizer symbolp
   :key-fixer null-symbol-fix
+  :key-equiv null-symbol-equiv
   :default-key nil
   :val-recognizer booleanp
   :val-fixer if-bool-fix
+  :val-equiv iff
   :default-val t)
 
 (atomic-stobjs::define-hash-table$a ht/0-boolean-nil eq
   :key-recognizer symbolp
   :key-fixer null-symbol-fix
+  :key-equiv null-symbol-equiv
   :default-key nil
   :val-recognizer booleanp
   :val-fixer if-bool-fix
+  :val-equiv iff
   :default-val t
   :copyable nil)
 
 (atomic-stobjs::define-hash-table$a ht/1-boolean eql
   :key-recognizer natp
   :key-fixer nfix
+  :key-equiv nat-equiv
   :default-key 0
   :val-recognizer booleanp
   :val-fixer if-bool-fix
+  :val-equiv iff
   :default-val t)
 
 (atomic-stobjs::define-hash-table$a ht/1-boolean-nil eql
   :key-recognizer natp
   :key-fixer nfix
+  :key-equiv nat-equiv
   :default-key 0
   :val-recognizer booleanp
   :val-fixer if-bool-fix
+  :val-equiv iff
   :default-val t
   :copyable nil)
 
 (atomic-stobjs::define-hash-table$a ht/2-boolean eql
   :key-recognizer characterp
   :key-fixer char-fix
+  :key-equiv char-equiv
   :default-key #.acl2::*null-char*
   :val-recognizer booleanp
   :val-fixer if-bool-fix
+  :val-equiv iff
   :default-val t)
 
 (atomic-stobjs::define-hash-table$a ht/2-boolean-nil eql
   :key-recognizer characterp
   :key-fixer char-fix
+  :key-equiv char-equiv
   :default-key #.acl2::*null-char*
   :val-recognizer booleanp
   :val-fixer if-bool-fix
+  :val-equiv iff
   :default-val t
   :copyable nil)
 
 (atomic-stobjs::define-hash-table$a ht/3-boolean hons-equal
   :val-recognizer booleanp
   :val-fixer if-bool-fix
+  :val-equiv iff
   :default-val t)
 
 (atomic-stobjs::define-hash-table$a ht/3-boolean-nil hons-equal
   :val-recognizer booleanp
   :val-fixer if-bool-fix
+  :val-equiv iff
   :default-val t
   :copyable nil)
 
 (atomic-stobjs::define-hash-table$a ht/4-boolean equal
   :val-recognizer booleanp
   :val-fixer if-bool-fix
+  :val-equiv iff
   :default-val t)
 
 (atomic-stobjs::define-hash-table$a ht/4-boolean-nil equal
   :val-recognizer booleanp
   :val-fixer if-bool-fix
+  :val-equiv iff
   :default-val t
   :copyable nil)
 
@@ -284,7 +344,9 @@
 (atomic-stobjs::define-hash-table$a ht-sym-sym eq
   :key-recognizer symbolp
   :key-fixer null-symbol-fix
+  :key-equiv null-symbol-equiv
   :default-key nil
   :val-recognizer symbolp
   :val-fixer null-symbol-fix
+  :val-equiv null-symbol-equiv
   :default-val nil)
